src/proof/algebra/reversed_reference.v
@@ -1,1311 +1,654 @@
 From New.proof Require Import prelude.
-From iris.algebra Require Import cmra gset.
+From iris.algebra Require Import cmra gmap gset.
 From iris.base_logic.lib Require Import own.
+From New.proof.algebra Require Import counted_reversed_reference.
 
 (*
-  reversed_reference is used to track the reference between objects in a state.
-  It is *reversed* because given an object k, reversed_reference tracks the set
-  of objects whose reference points to k. reversed_reference is implemented using
-  the view RA in Iris.
-
-  The auth is a map from key (K) to value (V), where each value has at most one
-  reference (R) pointing to another key in the map.
-
-  The frag is a map from reference to set of keys. For each reference, the set of
-  keys give us exactly the set of values in the auth that shares this reference.
-  The frag gives us the *reversed* reference.
-
-  Function f abstracts how to retrieve the reference from the value. Function g
-  abstracts how to convert the key and value into a reference that other values
-  might point to. In some simple cases where R equals K, g just returns the key and
-  ignores the value.
-
-  One usage of this resource algebra is to describe the parent reference (or owner
-  reference) mechanism in Kubernetes, where each object has at most one controller
-  owner. We often need to reason about the state of all children objects of a given
-  parent object, which is described by the frag. In this case, K is KKey.t, V is the
-  KObjectV.t, R is the product of KKey.t and UID.t, f returns the (only) controller
-  owner if it exists, and g returns the product of key and uid.
+  reversed_reference is the set-shaped specialization of
+  counted_reversed_reference. Each value extracts a set of references; the
+  counted core represents each set member with count 1. The public fragment
+  shape remains [r ↦ gset K].
 *)
 
-
-Section reversed_reference.
-Context (K : Type) `{Countable K} (R : Type) `{Countable R} (V : Type).
-Context (f : V → option R) (g : K → V → R).
-
-Definition authO : ofe := prodO (gmapO K (leibnizO V)) (gsetO (leibnizO R)).
+Section reversed_reference_frag.
+Context (K : Type) `{Countable K} (R : Type) `{Countable R}.
 
 Definition fragUR : ucmra := gmapUR R (prodR dfracR (agreeR (gset K))).
 
-Implicit Types (a : authO) (b : fragUR).
-Implicit Types (k : K) (r : R) (v : V) (n : nat).
-
-Local Definition proj_state a : gmap K V := fst a.
-Local Definition proj_used_reference a : gset R := snd a.
-
-Local Definition view_rel_raw n a b :=
-  (* each obj in a is a used reference *)
-  (map_Forall (λ k v, (g k v) ∈ (proj_used_reference a)) (proj_state a)) ∧
-  (* dfracs are valid *)
-  (map_Forall (λ _ '(dq, _), ✓ dq) b) ∧
-  (* for each (r, ks) in b, ks is the set of objects that point to r in a *)
-  (map_Forall (λ r '(_, agree_ks),
-    ∃ ks, agree_ks ≡ to_agree ks ∧ ks = dom (filter (λ '(_, v), f v = Some r) (proj_state a))) b) ∧
-  (* each r in b is a used reference *)
-  (map_Forall (λ r _, r ∈ (proj_used_reference a)) b).
-
-Local Lemma view_rel_raw_mono n1 n2 a1 a2 b1 b2 :
-  view_rel_raw n1 a1 b1 →
-  a1 ≡{n2}≡ a2 →
-  b2 ≼{n2} b1 →
-  (n2 ≤ n1)%nat →
-  view_rel_raw n2 a2 b2.
-Proof.
-  intros [Hobj [Hvalid [Hchildren Hreferences]]] Ha Hb _.
-  destruct a1 as [state1 used1], a2 as [state2 used2].
-  simpl in *.
-  destruct Ha as [Hstate Hused].
-  assert (Hstate_eqv : state1 ≡ state2).
-  { apply (proj2 (discrete_iff n2 state1 state2)).
-    exact Hstate.
-  }
-  assert (Hstate_eq : state1 = state2).
-  { change ((state1 : gmap K (leibnizO V)) =
-            (state2 : gmap K (leibnizO V))).
-    apply map_eq. intros k.
-    pose proof (proj1 (map_equiv_iff state1 state2) Hstate_eqv k) as Hlookup_eqv.
-    apply leibniz_equiv in Hlookup_eqv. done.
-  }
-  subst state2.
-  assert (Hused_eqv : used1 ≡ used2).
-  { apply (proj2 (discrete_iff n2 used1 used2)).
-    exact Hused.
-  }
-  assert (Hused_elem : ∀ r, r ∈ used1 ↔ r ∈ used2).
-  { exact (proj1 (set_equiv used1 used2) Hused_eqv). }
-  split.
-  - rewrite map_Forall_lookup.
-    intros k v Hlookup.
-    pose proof (map_Forall_lookup_1 _ _ _ _ Hobj Hlookup) as Hr_used1.
-    apply (proj1 (Hused_elem _)).
-    exact Hr_used1.
-  - split.
-    + rewrite map_Forall_lookup.
-      intros r [dq2 agree2] Hlookup2.
-      destruct (lookup_includedN n2 b2 b1) as [Hlookup_incl _].
-      specialize (Hlookup_incl Hb r).
-      rewrite Hlookup2 in Hlookup_incl.
-      destruct (Some_includedN_is_Some _ _ _ Hlookup_incl) as [da1 Hlookup1].
-      destruct da1 as [dq1 agree1].
-      destruct (Hchildren _ _ Hlookup1) as (ks & Hagree1 & _).
-      pose proof (map_Forall_lookup_1 _ _ _ _ Hvalid Hlookup1) as Hvdq1.
-      rewrite Hlookup1 in Hlookup_incl.
-      assert (Hval1_n2 :
-        ✓{n2} (Some (dq1, agree1) : option (dfrac * agree (gset K)))).
-      { simpl. apply cmra_valid_validN.
-        apply pair_valid. split; [done|].
-        rewrite Hagree1. done.
-      }
-      assert (Hval2_n2 :
-        ✓{n2} (Some (dq2, agree2) : option (dfrac * agree (gset K)))).
-      { eapply cmra_validN_includedN.
-        - exact Hval1_n2.
-        - exact Hlookup_incl.
-      }
-      assert (Hvdq2_n2 : ✓{n2} dq2).
-      { apply (proj1 (pair_validN dq2 agree2 n2)).
-        simpl in Hval2_n2. done.
-      }
-      by apply (proj2 (cmra_discrete_valid_iff n2 dq2)).
-    + split.
-      * rewrite map_Forall_lookup.
-        intros r [dq2 agree2] Hlookup2.
-        destruct (lookup_includedN n2 b2 b1) as [Hlookup_incl _].
-        specialize (Hlookup_incl Hb r).
-        rewrite Hlookup2 in Hlookup_incl.
-        destruct (Some_includedN_is_Some _ _ _ Hlookup_incl) as [da1 Hlookup1].
-        destruct da1 as [dq1 agree1].
-        destruct (Hchildren _ _ Hlookup1) as (ks & Hagree1 & Hdom1).
-        rewrite Hlookup1 in Hlookup_incl.
-        pose proof (Some_pair_includedN _ _ _ _ _ Hlookup_incl) as [_ Hagree_opt_incl].
-        pose proof (proj1 (Some_includedN_total n2 agree2 agree1) Hagree_opt_incl)
-          as Hagree_incl.
-        assert (Hagree1_n2 : ✓{n2} agree1).
-        { rewrite Hagree1. done. }
-        pose proof (agree_valid_includedN n2 agree2 agree1 Hagree1_n2 Hagree_incl)
-          as Hagree2_n2.
-        exists ks.
-        split.
-        -- apply (proj2 (discrete_iff n2 agree2 (to_agree ks))).
-           etrans; [exact Hagree2_n2|exact (Hagree1 n2)].
-        -- done.
-      * rewrite map_Forall_lookup.
-        intros r da2 Hlookup2.
-        destruct (lookup_includedN n2 b2 b1) as [Hlookup_incl _].
-        specialize (Hlookup_incl Hb r).
-        rewrite Hlookup2 in Hlookup_incl.
-        destruct (Some_includedN_is_Some _ _ _ Hlookup_incl) as [da1 Hlookup1].
-        pose proof (map_Forall_lookup_1 _ _ _ _ Hreferences Hlookup1) as Hr_used1.
-        apply (proj1 (Hused_elem _)).
-        exact Hr_used1.
-Qed.
-
-Local Lemma view_rel_raw_valid n a b :
-  view_rel_raw n a b → ✓{n} b.
-Proof.
-  intros [_ [Hvalid [Hchildren _]]] r.
-  destruct (b !! r) as [[dq agree_ks]|] eqn:Hlookup.
-  - pose proof (map_Forall_lookup_1 _ _ _ _ Hvalid Hlookup) as Hvdq.
-    pose proof (map_Forall_lookup_1 _ _ _ _ Hchildren Hlookup) as Hchild.
-    destruct Hchild as (ks & Hagree & _).
-    rewrite Hlookup.
-    apply pair_validN. split.
-    + apply cmra_valid_validN. done.
-    + rewrite Hagree. done.
-  - rewrite Hlookup. done.
-Qed.
-
-Local Lemma view_rel_raw_unit n :
-  ∃ a, view_rel_raw n a ε.
-Proof.
-  exists ((∅ : gmap K V), (∅ : gset R)).
-  split_and!.
-  all: rewrite map_Forall_lookup; intros i x Hlookup;
-    rewrite lookup_empty in Hlookup; done.
-Qed.
-
-Local Canonical Structure view_rel :
-    view_rel authO fragUR :=
-  ViewRel view_rel_raw view_rel_raw_mono
-          view_rel_raw_valid view_rel_raw_unit.
-
-Definition cview_auth dq a : viewR view_rel := ●V{dq} a.
-Definition cview_frag b : viewR view_rel := ◯V b.
-Definition mk_frag (p: R) (dq: dfrac) (ks: gset K) : fragUR :=
+Definition mk_frag (p : R) (dq : dfrac) (ks : gset K) : fragUR :=
   {[p := (dq, to_agree ks)]}.
-Notation "●C a" := (cview_auth 1 a) (at level 20).
-Notation "◯C b" := (cview_frag b) (at level 20).
 
-Lemma auth_frag_valid a r dq ks:
-  ✓ (●C a ⋅ ◯C (mk_frag r dq ks)) →
-  ks = dom (filter (λ '(_, v), f v = Some r) (proj_state a)) ∧
-  r ∈ (proj_used_reference a).
+End reversed_reference_frag.
+
+Arguments fragUR _ {_ _} _ {_ _}.
+Arguments mk_frag {_ _ _ _ _ _} _ _ _.
+
+Section reversed_reference.
+Context (K : Type) `{Countable K} (R : Type) `{Countable R} (V : Type).
+Context (extract_reference_set : V → gset R) (to_reference : K → V → R).
+
+Definition reverse_index (state : gmap K V) (r : R) : gset K :=
+  dom (filter (λ '(_, v), r ∈ extract_reference_set v) state).
+
+Definition extract_reference_count (v : V) : gmap R nat :=
+  gset_to_gmap 1 (extract_reference_set v).
+
+Definition counted_reverse_index (state : gmap K V) (r : R) : gmap K nat :=
+  @counted_reversed_reference.reverse_index
+    K _ _ R _ _ V extract_reference_count state r.
+
+Lemma counted_reverse_index_eq state r :
+  counted_reverse_index state r = gset_to_gmap 1 (reverse_index state r).
 Proof.
-  intros Hvalid.
-  rewrite /cview_auth /cview_frag in Hvalid.
-  pose proof (proj1 (view_both_dfrac_valid view_rel 1 a (mk_frag r dq ks)) Hvalid)
-    as [_ Hrel].
-  specialize (Hrel 0ᵢ).
-  change (view_rel_raw 0ᵢ a (mk_frag r dq ks)) in Hrel.
-  destruct Hrel as [_ [_ [Hchildren Hreferences]]].
-  assert (Hlookup : mk_frag r dq ks !! r = Some (dq, to_agree ks)).
-  { rewrite /mk_frag lookup_singleton_eq //. }
-  destruct (Hchildren _ _ Hlookup) as (ks' & Hagree & Hdom).
-  assert (Hks_eqv : ks ≡ ks').
-  { apply (inj to_agree). by rewrite Hagree. }
-  apply leibniz_equiv in Hks_eqv. subst ks'.
-  split; [done|].
-  eapply Hreferences; done.
-Qed.
-
-Lemma create_reference a k v r ks cks:
-  (proj_state a) !! k = None →
-  f v = Some r →
-  g k v ≠ r → (* No self-parenting *)
-  dom (filter (λ '(_, v'), f v' = Some (g k v)) (proj_state a)) = cks →
-  g k v ∉ (proj_used_reference a) →
-  ●C a ⋅
-  ◯C (mk_frag r 1 ks) ~~>
-    ●C ((<[k := v]> (proj_state a)), ((proj_used_reference a) ∪ {[g k v]})) ⋅
-    ◯C (mk_frag r 1 (ks ∪ {[k]})) ⋅
-    ◯C (mk_frag (g k v) 1 cks).
-Proof.
-  intros Hak Hfr Hnself Hcks Hfresh.
-  rewrite -assoc /cview_frag -view_frag_op.
-  apply view_update.
-  intros n bf [Hobj [Hvalid [Hchildren Hreferences]]].
-  assert (Hbf_none_r : bf !! r = None).
-  { destruct (bf !! r) as [[dqf agf]|] eqn:Hbf; [|done].
-    exfalso.
-    assert (Hlookup :
-      (mk_frag r 1 ks ⋅ bf) !! r = Some ((DfracOwn 1, to_agree ks) ⋅ (dqf, agf))).
-    { rewrite lookup_op /mk_frag lookup_singleton_eq Hbf Some_op_opM //. }
-    pose proof (Hvalid _ _ Hlookup) as Hvdq.
-    simpl in Hvdq.
-    pose proof (dfrac_valid_own_l dqf 1 Hvdq) as Hlt.
-    apply (Qp.lt_nge 1 1) in Hlt.
-    apply Hlt. reflexivity.
-  }
-  assert (Hbf_none_g : bf !! (g k v) = None).
-  { destruct (bf !! (g k v)) as [da|] eqn:Hbf; [|done].
-    exfalso. apply Hfresh.
-    assert (Hlookup_old_g : (mk_frag r 1 ks ⋅ bf) !! (g k v) = Some da).
-    { rewrite lookup_op.
-      assert (Hnone_old_r : mk_frag r 1 ks !! (g k v) = None).
-      { rewrite /mk_frag lookup_singleton_ne; done. }
-      rewrite Hnone_old_r Hbf left_id //. }
-    eapply Hreferences; done.
-  }
-  assert (Hlookup_r_old :
-    (mk_frag r 1 ks ⋅ bf) !! r = Some (DfracOwn 1, to_agree ks)).
-  { rewrite lookup_op /mk_frag lookup_singleton_eq Hbf_none_r right_id //. }
-  assert (Hks_dom : ks = dom (filter (λ '(_, v0), f v0 = Some r) (proj_state a))).
-  { destruct (Hchildren _ _ Hlookup_r_old) as (ks' & Hagree & Hdom).
-    assert (Hks_eqv : ks ≡ ks').
-    { apply (inj to_agree). by rewrite Hagree. }
-    apply leibniz_equiv in Hks_eqv. subst ks'. done.
-  }
-  assert (Hr_used : r ∈ proj_used_reference a).
-  { eapply Hreferences; done. }
-
-  split_and!.
-  - rewrite map_Forall_lookup.
-    intros k0 v0 Hlookup0.
-    simpl in Hlookup0.
-    destruct (decide (k0 = k)) as [->|Hneq_k].
-    + apply lookup_insert_Some in Hlookup0.
-      destruct Hlookup0 as [[_ Hv0]|[Hneq _]].
-      * symmetry in Hv0. subst v0.
-        apply elem_of_union. right.
-        apply elem_of_singleton. reflexivity.
-      * exfalso. apply Hneq. reflexivity.
-    + apply lookup_insert_Some in Hlookup0.
-      destruct Hlookup0 as [[Heq _]|[_ Hlookup_old]].
-      * exfalso. apply Hneq_k. symmetry. exact Heq.
-      * pose proof (map_Forall_lookup_1 _ _ _ _ Hobj Hlookup_old) as Hobj_used.
-        apply elem_of_union. left. exact Hobj_used.
-  - intros r0 [dq agree_ks] Hb.
-    rewrite lookup_op in Hb.
-    destruct (decide (r0 = r)) as [->|Hneq_r].
-    + assert (Hlookup_rg_r :
-        (mk_frag r 1 (ks ∪ {[k]}) ⋅ mk_frag (g k v) 1 cks) !! r =
-        Some (DfracOwn 1, to_agree (ks ∪ {[k]}))).
-      { rewrite lookup_op /mk_frag lookup_singleton_eq.
-        assert (Hg_none_r : mk_frag (g k v) 1 cks !! r = None).
-        { rewrite /mk_frag lookup_singleton_ne; done. }
-        rewrite Hg_none_r right_id //. }
-      rewrite Hlookup_rg_r Hbf_none_r right_id in Hb.
-      inversion Hb; subst dq agree_ks. done.
-    + destruct (decide (r0 = g k v)) as [->|Hneq_g].
-      * assert (Hlookup_rg_g :
-          (mk_frag r 1 (ks ∪ {[k]}) ⋅ mk_frag (g k v) 1 cks) !! (g k v) =
-          Some (DfracOwn 1, to_agree cks)).
-        { rewrite lookup_op.
-          assert (Hr_none_g : mk_frag r 1 (ks ∪ {[k]}) !! (g k v) = None).
-          { rewrite /mk_frag lookup_singleton_ne; done. }
-          rewrite Hr_none_g /mk_frag lookup_singleton_eq left_id //. }
-        rewrite Hlookup_rg_g Hbf_none_g right_id in Hb.
-        inversion Hb; subst dq agree_ks. done.
-      * assert (Hlookup_rg_none :
-          (mk_frag r 1 (ks ∪ {[k]}) ⋅ mk_frag (g k v) 1 cks) !! r0 = None).
-        { rewrite lookup_op.
-          assert (Hr_none : mk_frag r 1 (ks ∪ {[k]}) !! r0 = None).
-          { rewrite /mk_frag lookup_singleton_ne; done. }
-          assert (Hg_none : mk_frag (g k v) 1 cks !! r0 = None).
-          { rewrite /mk_frag lookup_singleton_ne; done. }
-          rewrite Hr_none Hg_none left_id //. }
-        rewrite Hlookup_rg_none in Hb.
-        rewrite left_id in Hb.
-        assert (Hlookup_old : (mk_frag r 1 ks ⋅ bf) !! r0 = Some (dq, agree_ks)).
-        { rewrite lookup_op.
-          assert (Hnone_old : mk_frag r 1 ks !! r0 = None).
-          { rewrite /mk_frag lookup_singleton_ne; done. }
-          rewrite Hnone_old Hb left_id //. }
-        exact (map_Forall_lookup_1
-          (λ _ '(dq0, _), ✓ dq0)
-          (mk_frag r 1 ks ⋅ bf) r0 (dq, agree_ks)
-          Hvalid Hlookup_old).
-  - intros r0 [dq agree_ks] Hb.
-    rewrite lookup_op in Hb.
-    destruct (decide (r0 = r)) as [->|Hneq_r].
-    + assert (Hlookup_rg_r :
-        (mk_frag r 1 (ks ∪ {[k]}) ⋅ mk_frag (g k v) 1 cks) !! r =
-        Some (DfracOwn 1, to_agree (ks ∪ {[k]}))).
-      { rewrite lookup_op /mk_frag lookup_singleton_eq.
-        assert (Hg_none_r : mk_frag (g k v) 1 cks !! r = None).
-        { rewrite /mk_frag lookup_singleton_ne; done. }
-        rewrite Hg_none_r right_id //. }
-      rewrite Hlookup_rg_r Hbf_none_r right_id in Hb.
-      inversion Hb; subst dq agree_ks.
-      exists (ks ∪ {[k]}). split; [done|].
-      assert (Hfins :
-        filter (λ '(_, v0), f v0 = Some r) (<[k := v]> (proj_state a)) =
-        <[k := v]> (filter (λ '(_, v0), f v0 = Some r) (proj_state a))).
-      { apply map_filter_insert_True.
-        rewrite Hfr. done.
-      }
-      rewrite Hfins dom_insert_L Hks_dom union_comm_L //.
-    + destruct (decide (r0 = g k v)) as [->|Hneq_g].
-      * assert (Hlookup_rg_g :
-          (mk_frag r 1 (ks ∪ {[k]}) ⋅ mk_frag (g k v) 1 cks) !! (g k v) =
-          Some (DfracOwn 1, to_agree cks)).
-        { rewrite lookup_op.
-          assert (Hr_none_g : mk_frag r 1 (ks ∪ {[k]}) !! (g k v) = None).
-          { rewrite /mk_frag lookup_singleton_ne; done. }
-          rewrite Hr_none_g /mk_frag lookup_singleton_eq left_id //. }
-        rewrite Hlookup_rg_g Hbf_none_g right_id in Hb.
-        inversion Hb; subst dq agree_ks.
-        exists cks. split; [done|].
-        assert (Hfins :
-          filter (λ '(_, v0), f v0 = Some (g k v)) (<[k := v]> (proj_state a)) =
-          filter (λ '(_, v0), f v0 = Some (g k v)) (proj_state a)).
-        { apply map_filter_insert_not'.
-          - rewrite Hfr. intros Hcontra. inversion Hcontra. subst. done.
-          - intros y Hy. rewrite Hak in Hy. done.
-        }
-        rewrite Hfins Hcks. done.
-      * assert (Hlookup_rg_none :
-          (mk_frag r 1 (ks ∪ {[k]}) ⋅ mk_frag (g k v) 1 cks) !! r0 = None).
-        { rewrite lookup_op.
-          assert (Hr_none : mk_frag r 1 (ks ∪ {[k]}) !! r0 = None).
-          { rewrite /mk_frag lookup_singleton_ne; done. }
-          assert (Hg_none : mk_frag (g k v) 1 cks !! r0 = None).
-          { rewrite /mk_frag lookup_singleton_ne; done. }
-          rewrite Hr_none Hg_none left_id //. }
-        rewrite Hlookup_rg_none in Hb.
-        rewrite left_id in Hb.
-        assert (Hlookup_old : (mk_frag r 1 ks ⋅ bf) !! r0 = Some (dq, agree_ks)).
-        { rewrite lookup_op.
-          assert (Hnone_old : mk_frag r 1 ks !! r0 = None).
-          { rewrite /mk_frag lookup_singleton_ne; done. }
-          rewrite Hnone_old Hb left_id //. }
-        destruct (Hchildren _ _ Hlookup_old) as (ks0 & Hagree & Hdom).
-        exists ks0. split; [done|].
-        assert (Hfins :
-          filter (λ '(_, v0), f v0 = Some r0) (<[k := v]> (proj_state a)) =
-          filter (λ '(_, v0), f v0 = Some r0) (proj_state a)).
-        { apply map_filter_insert_not'.
-          - rewrite Hfr. intros Hcontra. inversion Hcontra. subst. done.
-          - intros y Hy. rewrite Hak in Hy. done.
-        }
-        rewrite Hfins. done.
-  - intros r0 da Hb.
-    rewrite lookup_op in Hb.
-    destruct (decide (r0 = r)) as [->|Hneq_r].
-    + set_solver.
-    + destruct (decide (r0 = g k v)) as [->|Hneq_g].
-      * set_solver.
-      * assert (Hlookup_rg_none :
-          (mk_frag r 1 (ks ∪ {[k]}) ⋅ mk_frag (g k v) 1 cks) !! r0 = None).
-        { rewrite lookup_op.
-          assert (Hr_none : mk_frag r 1 (ks ∪ {[k]}) !! r0 = None).
-          { rewrite /mk_frag lookup_singleton_ne; done. }
-          assert (Hg_none : mk_frag (g k v) 1 cks !! r0 = None).
-          { rewrite /mk_frag lookup_singleton_ne; done. }
-          rewrite Hr_none Hg_none left_id //. }
-        rewrite Hlookup_rg_none in Hb.
-        rewrite left_id in Hb.
-        assert (Hlookup_old : (mk_frag r 1 ks ⋅ bf) !! r0 = Some da).
-        { rewrite lookup_op.
-          assert (Hnone_old : mk_frag r 1 ks !! r0 = None).
-          { rewrite /mk_frag lookup_singleton_ne; done. }
-          rewrite Hnone_old Hb left_id //. }
-        specialize (Hreferences _ _ Hlookup_old). set_solver.
-Qed.
-
-Lemma set_reference a k v r ks v':
-  (proj_state a) !! k = Some v →
-  f v = None →
-  f v' = Some r →
-  g k v = g k v' →
-  ●C a ⋅
-  ◯C (mk_frag r 1 ks) ~~>
-    ●C ((<[k := v']> (proj_state a)), (proj_used_reference a)) ⋅
-    ◯C (mk_frag r 1 (ks ∪ {[k]})).
-Proof.
-  intros Hak Hnone Hfr Hg.
-  apply view_update.
-  intros n bf [Hobj [Hvalid [Hchildren Hreferences]]].
-  assert (Hbf_none : bf !! r = None).
-  { destruct (bf !! r) as [[dqf agf]|] eqn:Hbf; [|done].
-    exfalso.
-    assert (Hlookup :
-      (mk_frag r 1 ks ⋅ bf) !! r = Some ((DfracOwn 1, to_agree ks) ⋅ (dqf, agf))).
-    { rewrite lookup_op /mk_frag lookup_singleton_eq Hbf Some_op_opM //. }
-    pose proof (Hvalid _ _ Hlookup) as Hvdq.
-    simpl in Hvdq.
-    pose proof (dfrac_valid_own_l dqf 1 Hvdq) as Hlt.
-    apply (Qp.lt_nge 1 1) in Hlt.
-    apply Hlt. done.
-  }
-  assert (Hlookup_r_old :
-    (mk_frag r 1 ks ⋅ bf) !! r = Some (DfracOwn 1, to_agree ks)).
-  { rewrite lookup_op /mk_frag lookup_singleton_eq Hbf_none right_id //. }
-  assert (Hks_dom : ks = dom (filter (λ '(_, v0), f v0 = Some r) (proj_state a))).
-  { destruct (Hchildren _ _ Hlookup_r_old) as (ks' & Hagree & Hdom).
-    assert (Hks_eqv : ks ≡ ks').
-    { apply (inj to_agree). by rewrite Hagree. }
-    apply leibniz_equiv in Hks_eqv. subst ks'. done.
-  }
-  assert (Hr_used : r ∈ proj_used_reference a).
-  { eapply Hreferences; done. }
-  assert (Hdom_transfer :
-    ∀ x,
-      x ∈ dom (mk_frag r 1 ks ⋅ bf) →
-      x ∈ dom (mk_frag r 1 (ks ∪ {[k]}) ⋅ bf)).
-  { intros x Hx.
-    destruct (decide (x = r)) as [->|Hneq_x].
-    - apply elem_of_dom_2 with (x := (DfracOwn 1, to_agree (ks ∪ {[k]}))).
-      rewrite lookup_op /mk_frag lookup_singleton_eq Hbf_none right_id //.
-    - rewrite elem_of_dom in Hx.
-      destruct Hx as [da Hlookup_old].
-      assert (Hbf_lookup : bf !! x = Some da).
-      { rewrite lookup_op in Hlookup_old.
-        assert (Hnone_old : mk_frag r 1 ks !! x = None).
-        { rewrite /mk_frag lookup_singleton_ne; done. }
-        rewrite Hnone_old left_id in Hlookup_old. done.
-      }
-      apply elem_of_dom_2 with (x := da).
-      rewrite lookup_op.
-      assert (Hnone_new : mk_frag r 1 (ks ∪ {[k]}) !! x = None).
-      { rewrite /mk_frag lookup_singleton_ne; done. }
-      rewrite Hnone_new Hbf_lookup left_id //.
-  }
-
-  split_and!.
-  - rewrite map_Forall_lookup.
-    intros k0 v0 Hlookup0.
-    simpl in Hlookup0.
-    destruct (decide (k0 = k)) as [->|Hneq_k].
-    + apply lookup_insert_Some in Hlookup0.
-      destruct Hlookup0 as [[_ Hv0]|[Hneq _]].
-      * symmetry in Hv0. subst v0.
-        rewrite <- Hg.
-        exact (map_Forall_lookup_1 _ _ _ _ Hobj Hak).
-      * exfalso. apply Hneq. reflexivity.
-    + apply lookup_insert_Some in Hlookup0.
-      destruct Hlookup0 as [[Heq _]|[_ Hlookup_old]].
-      * exfalso. apply Hneq_k. symmetry. exact Heq.
-      * exact (map_Forall_lookup_1 _ _ _ _ Hobj Hlookup_old).
-  - intros r0 [dq agree_ks] Hb.
-    rewrite lookup_op in Hb.
-    destruct (decide (r0 = r)) as [->|Hneq].
-    + rewrite /mk_frag lookup_singleton_eq Hbf_none right_id in Hb.
-      inversion Hb; subst dq agree_ks. done.
-    + assert (Hlookup_new : mk_frag r 1 (ks ∪ {[k]}) !! r0 = None).
-      { rewrite /mk_frag lookup_singleton_ne; done. }
-      rewrite Hlookup_new in Hb.
-      rewrite left_id in Hb.
-      assert (Hlookup_old : (mk_frag r 1 ks ⋅ bf) !! r0 = Some (dq, agree_ks)).
-      { rewrite lookup_op.
-        assert (Hnone_old : mk_frag r 1 ks !! r0 = None).
-        { rewrite /mk_frag lookup_singleton_ne; done. }
-        rewrite Hnone_old Hb left_id //. }
-      exact (map_Forall_lookup_1
-        (λ _ '(dq0, _), ✓ dq0)
-        (mk_frag r 1 ks ⋅ bf) r0 (dq, agree_ks)
-        Hvalid Hlookup_old).
-  - intros r0 [dq agree_ks] Hb.
-    rewrite lookup_op in Hb.
-    destruct (decide (r0 = r)) as [->|Hneq].
-    + rewrite /mk_frag lookup_singleton_eq Hbf_none right_id in Hb.
-      inversion Hb; subst dq agree_ks.
-      exists (ks ∪ {[k]}). split; [done|].
-      assert (Hfins :
-        filter (λ '(_, v0), f v0 = Some r) (<[k := v']> (proj_state a)) =
-        <[k := v']> (filter (λ '(_, v0), f v0 = Some r) (proj_state a))).
-      { apply map_filter_insert_True.
-        rewrite Hfr. done.
-      }
-      rewrite Hfins dom_insert_L Hks_dom union_comm_L //.
-    + assert (Hlookup_new : mk_frag r 1 (ks ∪ {[k]}) !! r0 = None).
-      { rewrite /mk_frag lookup_singleton_ne; done. }
-      rewrite Hlookup_new in Hb.
-      rewrite left_id in Hb.
-      assert (Hlookup_old : (mk_frag r 1 ks ⋅ bf) !! r0 = Some (dq, agree_ks)).
-      { rewrite lookup_op.
-        assert (Hnone_old : mk_frag r 1 ks !! r0 = None).
-        { rewrite /mk_frag lookup_singleton_ne; done. }
-        rewrite Hnone_old Hb left_id //. }
-      destruct (Hchildren _ _ Hlookup_old) as (ks0 & Hagree & Hdom).
-      exists ks0. split; [done|].
-      assert (Hfins :
-        filter (λ '(_, v0), f v0 = Some r0) (<[k := v']> (proj_state a)) =
-        filter (λ '(_, v0), f v0 = Some r0) (proj_state a)).
-      { apply map_filter_insert_not'.
-        - rewrite Hfr. intros Hcontra. inversion Hcontra. subst. done.
-        - intros y Hy.
-          rewrite Hak in Hy. inversion Hy; subst.
-          rewrite Hnone. discriminate.
-      }
-      rewrite Hfins. done.
-  - intros r0 da Hb.
-    destruct (decide (r0 = r)) as [->|Hneq].
-    + done.
-    + rewrite lookup_op in Hb.
-      assert (Hlookup_new : mk_frag r 1 (ks ∪ {[k]}) !! r0 = None).
-      { rewrite /mk_frag lookup_singleton_ne; done. }
-      rewrite Hlookup_new in Hb.
-      rewrite left_id in Hb.
-      assert (Hlookup_old : (mk_frag r 1 ks ⋅ bf) !! r0 = Some da).
-      { rewrite lookup_op.
-        assert (Hnone_old : mk_frag r 1 ks !! r0 = None).
-        { rewrite /mk_frag lookup_singleton_ne; done. }
-        rewrite Hnone_old Hb left_id //. }
-      eapply Hreferences; done.
-Qed.
-
-Lemma unset_reference a k v r ks v':
-  (proj_state a) !! k = Some v →
-  f v = Some r →
-  f v' = None →
-  g k v = g k v' →
-  ●C a ⋅
-  ◯C (mk_frag r 1 ks) ~~>
-    ●C ((<[k := v']> (proj_state a)), (proj_used_reference a)) ⋅
-    ◯C (mk_frag r 1 (ks ∖ {[k]})).
-Proof.
-  intros Hak Hfr Hnone Hg.
-  apply view_update.
-  intros n bf [Hobj [Hvalid [Hchildren Hreferences]]].
-  assert (Hbf_none : bf !! r = None).
-  { destruct (bf !! r) as [[dqf agf]|] eqn:Hbf; [|done].
-    exfalso.
-    assert (Hlookup :
-      (mk_frag r 1 ks ⋅ bf) !! r = Some ((DfracOwn 1, to_agree ks) ⋅ (dqf, agf))).
-    { rewrite lookup_op /mk_frag lookup_singleton_eq Hbf Some_op_opM //. }
-    pose proof (Hvalid _ _ Hlookup) as Hvdq.
-    simpl in Hvdq.
-    pose proof (dfrac_valid_own_l dqf 1 Hvdq) as Hlt.
-    apply (Qp.lt_nge 1 1) in Hlt.
-    apply Hlt. reflexivity.
-  }
-  assert (Hlookup_r_old :
-    (mk_frag r 1 ks ⋅ bf) !! r = Some (DfracOwn 1, to_agree ks)).
-  { rewrite lookup_op /mk_frag lookup_singleton_eq Hbf_none right_id //. }
-  assert (Hks_dom : ks = dom (filter (λ '(_, v0), f v0 = Some r) (proj_state a))).
-  { destruct (Hchildren _ _ Hlookup_r_old) as (ks' & Hagree & Hdom).
-    assert (Hks_eqv : ks ≡ ks').
-    { apply (inj to_agree). by rewrite Hagree. }
-    apply leibniz_equiv in Hks_eqv. subst ks'. done.
-  }
-  assert (Hr_used : r ∈ proj_used_reference a).
-  { eapply Hreferences; done. }
-  assert (Hdom_transfer :
-    ∀ x,
-      x ∈ dom (mk_frag r 1 ks ⋅ bf) →
-      x ∈ dom (mk_frag r 1 (ks ∖ {[k]}) ⋅ bf)).
-  { intros x Hx.
-    destruct (decide (x = r)) as [->|Hneq_x].
-    - apply elem_of_dom_2 with (x := (DfracOwn 1, to_agree (ks ∖ {[k]}))).
-      rewrite lookup_op /mk_frag lookup_singleton_eq Hbf_none right_id //.
-    - rewrite elem_of_dom in Hx.
-      destruct Hx as [da Hlookup_old].
-      assert (Hbf_lookup : bf !! x = Some da).
-      { rewrite lookup_op in Hlookup_old.
-        assert (Hnone_old : mk_frag r 1 ks !! x = None).
-        { rewrite /mk_frag lookup_singleton_ne; done. }
-        rewrite Hnone_old left_id in Hlookup_old. done.
-      }
-      apply elem_of_dom_2 with (x := da).
-      rewrite lookup_op.
-      assert (Hnone_new : mk_frag r 1 (ks ∖ {[k]}) !! x = None).
-      { rewrite /mk_frag lookup_singleton_ne; done. }
-      rewrite Hnone_new Hbf_lookup left_id //.
-  }
-
-  repeat split.
-  - rewrite map_Forall_lookup.
-    intros k0 v0 Hlookup0.
-    simpl in Hlookup0.
-    destruct (decide (k0 = k)) as [->|Hneq_k].
-    + apply lookup_insert_Some in Hlookup0.
-      destruct Hlookup0 as [[_ Hv0]|[Hneq _]].
-      * symmetry in Hv0. subst v0.
-        rewrite <- Hg.
-        exact (map_Forall_lookup_1 _ _ _ _ Hobj Hak).
-      * exfalso. apply Hneq. reflexivity.
-    + apply lookup_insert_Some in Hlookup0.
-      destruct Hlookup0 as [[Heq _]|[_ Hlookup_old]].
-      * exfalso. apply Hneq_k. symmetry. exact Heq.
-      * exact (map_Forall_lookup_1 _ _ _ _ Hobj Hlookup_old).
-  - intros r0 [dq agree_ks] Hb.
-    rewrite lookup_op in Hb.
-    destruct (decide (r0 = r)) as [->|Hneq].
-    + rewrite /mk_frag lookup_singleton_eq Hbf_none right_id in Hb.
-      inversion Hb; subst dq agree_ks. done.
-    + assert (Hlookup_new : mk_frag r 1 (ks ∖ {[k]}) !! r0 = None).
-      { rewrite /mk_frag lookup_singleton_ne; done. }
-      rewrite Hlookup_new in Hb.
-      rewrite left_id in Hb.
-      assert (Hlookup_old : (mk_frag r 1 ks ⋅ bf) !! r0 = Some (dq, agree_ks)).
-      { rewrite lookup_op.
-        assert (Hnone_old : mk_frag r 1 ks !! r0 = None).
-        { rewrite /mk_frag lookup_singleton_ne; done. }
-        rewrite Hnone_old Hb left_id //. }
-      exact (map_Forall_lookup_1
-        (λ _ '(dq0, _), ✓ dq0)
-        (mk_frag r 1 ks ⋅ bf) r0 (dq, agree_ks)
-        Hvalid Hlookup_old).
-  - intros r0 [dq agree_ks] Hb.
-    rewrite lookup_op in Hb.
-    destruct (decide (r0 = r)) as [->|Hneq].
-    + rewrite /mk_frag lookup_singleton_eq Hbf_none right_id in Hb.
-      inversion Hb; subst dq agree_ks.
-      exists (ks ∖ {[k]}). split; [done|].
-      assert (Hfins :
-        filter (λ '(_, v0), f v0 = Some r) (<[k := v']> (proj_state a)) =
-        filter (λ '(_, v0), f v0 = Some r) (delete k (proj_state a))).
-      { apply map_filter_insert_False.
-        rewrite Hnone. discriminate.
-      }
-      assert (Hfdel :
-        filter (λ '(_, v0), f v0 = Some r) (delete k (proj_state a)) =
-        delete k (filter (λ '(_, v0), f v0 = Some r) (proj_state a))).
-      { apply map_filter_delete. }
-      rewrite Hfins Hfdel dom_delete_L Hks_dom. done.
-    + assert (Hlookup_new : mk_frag r 1 (ks ∖ {[k]}) !! r0 = None).
-      { rewrite /mk_frag lookup_singleton_ne; done. }
-      rewrite Hlookup_new in Hb.
-      rewrite left_id in Hb.
-      assert (Hlookup_old : (mk_frag r 1 ks ⋅ bf) !! r0 = Some (dq, agree_ks)).
-      { rewrite lookup_op.
-        assert (Hnone_old : mk_frag r 1 ks !! r0 = None).
-        { rewrite /mk_frag lookup_singleton_ne; done. }
-        rewrite Hnone_old Hb left_id //. }
-      destruct (Hchildren _ _ Hlookup_old) as (ks0 & Hagree & Hdom).
-      exists ks0. split; [done|].
-      assert (Hfins :
-        filter (λ '(_, v0), f v0 = Some r0) (<[k := v']> (proj_state a)) =
-        filter (λ '(_, v0), f v0 = Some r0) (proj_state a)).
-      { apply map_filter_insert_not'.
-        - rewrite Hnone. discriminate.
-        - intros y Hy.
-          rewrite Hak in Hy. inversion Hy; subst.
-          rewrite Hfr. intros Hcontra.
-          inversion Hcontra. subst. done.
-      }
-      rewrite Hfins. done.
-  - intros r0 da Hb.
-    destruct (decide (r0 = r)) as [->|Hneq].
-    + done.
-    + rewrite lookup_op in Hb.
-      assert (Hlookup_new : mk_frag r 1 (ks ∖ {[k]}) !! r0 = None).
-      { rewrite /mk_frag lookup_singleton_ne; done. }
-      rewrite Hlookup_new in Hb.
-      rewrite left_id in Hb.
-      assert (Hlookup_old : (mk_frag r 1 ks ⋅ bf) !! r0 = Some da).
-      { rewrite lookup_op.
-        assert (Hnone_old : mk_frag r 1 ks !! r0 = None).
-        { rewrite /mk_frag lookup_singleton_ne; done. }
-        rewrite Hnone_old Hb left_id //. }
-      eapply Hreferences; done.
-Qed.
-
-Lemma delete_reference a k v r ks:
-  (proj_state a) !! k = Some v →
-  f v = Some r →
-  ●C a ⋅
-  ◯C (mk_frag r 1 ks) ~~>
-    ●C ((delete k (proj_state a)), (proj_used_reference a)) ⋅
-    ◯C (mk_frag r 1 (ks ∖ {[k]})).
-Proof.
-  intros Hak Hfr.
-  apply view_update.
-  intros n bf [Hobj [Hvalid [Hchildren Hreferences]]].
-  assert (Hbf_none : bf !! r = None).
-  { destruct (bf !! r) as [[dqf agf]|] eqn:Hbf; [|done].
-    exfalso.
-    assert (Hlookup :
-      (mk_frag r 1 ks ⋅ bf) !! r = Some ((DfracOwn 1, to_agree ks) ⋅ (dqf, agf))).
-    { rewrite lookup_op /mk_frag lookup_singleton_eq Hbf Some_op_opM //. }
-    pose proof (Hvalid _ _ Hlookup) as Hvdq.
-    simpl in Hvdq.
-    pose proof (dfrac_valid_own_l dqf 1 Hvdq) as Hlt.
-    apply (Qp.lt_nge 1 1) in Hlt.
-    apply Hlt. reflexivity.
-  }
-  assert (Hlookup_r_old :
-    (mk_frag r 1 ks ⋅ bf) !! r = Some (DfracOwn 1, to_agree ks)).
-  { rewrite lookup_op /mk_frag lookup_singleton_eq Hbf_none right_id //. }
-  assert (Hks_dom : ks = dom (filter (λ '(_, v0), f v0 = Some r) (proj_state a))).
-  { destruct (Hchildren _ _ Hlookup_r_old) as (ks' & Hagree & Hdom).
-    assert (Hks_eqv : ks ≡ ks').
-    { apply (inj to_agree). by rewrite Hagree. }
-    apply leibniz_equiv in Hks_eqv. subst ks'. done.
-  }
-  assert (Hr_used : r ∈ proj_used_reference a).
-  { eapply Hreferences; done. }
-  assert (Hdom_transfer :
-    ∀ x,
-      x ∈ dom (mk_frag r 1 ks ⋅ bf) →
-      x ∈ dom (mk_frag r 1 (ks ∖ {[k]}) ⋅ bf)).
-  { intros x Hx.
-    destruct (decide (x = r)) as [->|Hneq_x].
-    - apply elem_of_dom_2 with (x := (DfracOwn 1, to_agree (ks ∖ {[k]}))).
-      rewrite lookup_op /mk_frag lookup_singleton_eq Hbf_none right_id //.
-    - rewrite elem_of_dom in Hx.
-      destruct Hx as [da Hlookup_old].
-      assert (Hbf_lookup : bf !! x = Some da).
-      { rewrite lookup_op in Hlookup_old.
-        assert (Hnone_old : mk_frag r 1 ks !! x = None).
-        { rewrite /mk_frag lookup_singleton_ne; done. }
-        rewrite Hnone_old left_id in Hlookup_old. done.
-      }
-      apply elem_of_dom_2 with (x := da).
-      rewrite lookup_op.
-      assert (Hnone_new : mk_frag r 1 (ks ∖ {[k]}) !! x = None).
-      { rewrite /mk_frag lookup_singleton_ne; done. }
-      rewrite Hnone_new Hbf_lookup left_id //.
-  }
-
-  repeat split.
-  - rewrite map_Forall_lookup.
-    intros k0 v0 Hlookup0.
-    simpl in Hlookup0.
-    apply lookup_delete_Some in Hlookup0 as [_ Hlookup_old].
-    exact (map_Forall_lookup_1 _ _ _ _ Hobj Hlookup_old).
-  - intros r0 [dq agree_ks] Hb.
-    rewrite lookup_op in Hb.
-    destruct (decide (r0 = r)) as [->|Hneq].
-    + rewrite /mk_frag lookup_singleton_eq Hbf_none right_id in Hb.
-      inversion Hb; subst dq agree_ks. done.
-    + assert (Hlookup_new : mk_frag r 1 (ks ∖ {[k]}) !! r0 = None).
-      { rewrite /mk_frag lookup_singleton_ne; done. }
-      rewrite Hlookup_new in Hb.
-      rewrite left_id in Hb.
-      assert (Hlookup_old : (mk_frag r 1 ks ⋅ bf) !! r0 = Some (dq, agree_ks)).
-      { rewrite lookup_op.
-        assert (Hnone_old : mk_frag r 1 ks !! r0 = None).
-        { rewrite /mk_frag lookup_singleton_ne; done. }
-        rewrite Hnone_old Hb left_id //. }
-      exact (map_Forall_lookup_1
-        (λ _ '(dq0, _), ✓ dq0)
-        (mk_frag r 1 ks ⋅ bf) r0 (dq, agree_ks)
-        Hvalid Hlookup_old).
-  - intros r0 [dq agree_ks] Hb.
-    rewrite lookup_op in Hb.
-    destruct (decide (r0 = r)) as [->|Hneq].
-    + rewrite /mk_frag lookup_singleton_eq Hbf_none right_id in Hb.
-      inversion Hb; subst dq agree_ks.
-      exists (ks ∖ {[k]}). split; [done|].
-      assert (Hfdel :
-        filter (λ '(_, v0), f v0 = Some r) (delete k (proj_state a)) =
-        delete k (filter (λ '(_, v0), f v0 = Some r) (proj_state a))).
-      { apply map_filter_delete. }
-      rewrite Hfdel dom_delete_L Hks_dom. done.
-    + assert (Hlookup_new : mk_frag r 1 (ks ∖ {[k]}) !! r0 = None).
-      { rewrite /mk_frag lookup_singleton_ne; done. }
-      rewrite Hlookup_new in Hb.
-      rewrite left_id in Hb.
-      assert (Hlookup_old : (mk_frag r 1 ks ⋅ bf) !! r0 = Some (dq, agree_ks)).
-      { rewrite lookup_op.
-        assert (Hnone_old : mk_frag r 1 ks !! r0 = None).
-        { rewrite /mk_frag lookup_singleton_ne; done. }
-        rewrite Hnone_old Hb left_id //. }
-      destruct (Hchildren _ _ Hlookup_old) as (ks0 & Hagree & Hdom).
-      exists ks0. split; [done|].
-      assert (Hfdel :
-        filter (λ '(_, v0), f v0 = Some r0) (delete k (proj_state a)) =
-        filter (λ '(_, v0), f v0 = Some r0) (proj_state a)).
-      { change
-          ((filter (λ '(_, v0), f v0 = Some r0) (delete k (proj_state a)) : gmap K (leibnizO V)) =
-           (filter (λ '(_, v0), f v0 = Some r0) (proj_state a) : gmap K (leibnizO V))).
-        refine (@map_filter_delete_not K (gmap K)
-          _ _ _ _ _ _ _ _ _ (leibnizO V)
-          (λ '(_, v0), f v0 = Some r0) _ (proj_state a) k _).
-        intros y Hy.
-        rewrite Hak in Hy. inversion Hy; subst.
-        rewrite Hfr. intros Hcontra.
-        inversion Hcontra. subst. done.
-      }
-      rewrite Hfdel. done.
-  - intros r0 da Hb.
-    destruct (decide (r0 = r)) as [->|Hneq].
-    + done.
-    + rewrite lookup_op in Hb.
-      assert (Hlookup_new : mk_frag r 1 (ks ∖ {[k]}) !! r0 = None).
-      { rewrite /mk_frag lookup_singleton_ne; done. }
-      rewrite Hlookup_new in Hb.
-      rewrite left_id in Hb.
-      assert (Hlookup_old : (mk_frag r 1 ks ⋅ bf) !! r0 = Some da).
-      { rewrite lookup_op.
-        assert (Hnone_old : mk_frag r 1 ks !! r0 = None).
-        { rewrite /mk_frag lookup_singleton_ne; done. }
-        rewrite Hnone_old Hb left_id //. }
-      eapply Hreferences; done.
-Qed.
-
-Lemma delete_reference2 a k r ks:
-  k ∈ ks →
-  ●C a ⋅
-  ◯C (mk_frag r 1 ks) ~~>
-    ●C ((delete k (proj_state a)), (proj_used_reference a)) ⋅
-    ◯C (mk_frag r 1 (ks ∖ {[k]})).
-Proof.
-  intros Hk.
-  apply view_update.
-  intros n bf [Hobj [Hvalid [Hchildren Hreferences]]].
-  assert (Hbf_none : bf !! r = None).
-  { destruct (bf !! r) as [[dqf agf]|] eqn:Hbf; [|done].
-    exfalso.
-    assert (Hlookup :
-      (mk_frag r 1 ks ⋅ bf) !! r = Some ((DfracOwn 1, to_agree ks) ⋅ (dqf, agf))).
-    { rewrite lookup_op /mk_frag lookup_singleton_eq Hbf Some_op_opM //. }
-    pose proof (Hvalid _ _ Hlookup) as Hvdq.
-    simpl in Hvdq.
-    pose proof (dfrac_valid_own_l dqf 1 Hvdq) as Hlt.
-    apply (Qp.lt_nge 1 1) in Hlt.
-    apply Hlt. reflexivity.
-  }
-  assert (Hlookup_r_old :
-    (mk_frag r 1 ks ⋅ bf) !! r = Some (DfracOwn 1, to_agree ks)).
-  { rewrite lookup_op /mk_frag lookup_singleton_eq Hbf_none right_id //. }
-  assert (Hks_dom : ks = dom (filter (λ '(_, v0), f v0 = Some r) (proj_state a))).
-  { destruct (Hchildren _ _ Hlookup_r_old) as (ks' & Hagree & Hdom).
-    assert (Hks_eqv : ks ≡ ks').
-    { apply (inj to_agree). by rewrite Hagree. }
-    apply leibniz_equiv in Hks_eqv. subst ks'. done.
-  }
-  assert (Hr_used : r ∈ proj_used_reference a).
-  { eapply Hreferences; done. }
-  assert (Hk_in_dom : k ∈ dom (filter (λ '(_, v0), f v0 = Some r) (proj_state a))).
-  { rewrite -Hks_dom. done. }
-  apply elem_of_dom in Hk_in_dom as [vk Hk_lookup].
-  apply map_lookup_filter_Some in Hk_lookup as [Hak Hfkr].
-  assert (Hdom_transfer :
-    ∀ x,
-      x ∈ dom (mk_frag r 1 ks ⋅ bf) →
-      x ∈ dom (mk_frag r 1 (ks ∖ {[k]}) ⋅ bf)).
-  { intros x Hx.
-    destruct (decide (x = r)) as [->|Hneq_x].
-    - apply elem_of_dom_2 with (x := (DfracOwn 1, to_agree (ks ∖ {[k]}))).
-      rewrite lookup_op /mk_frag lookup_singleton_eq Hbf_none right_id //.
-    - rewrite elem_of_dom in Hx.
-      destruct Hx as [da Hlookup_old].
-      assert (Hbf_lookup : bf !! x = Some da).
-      { rewrite lookup_op in Hlookup_old.
-        assert (Hnone_old : mk_frag r 1 ks !! x = None).
-        { rewrite /mk_frag lookup_singleton_ne; done. }
-        rewrite Hnone_old left_id in Hlookup_old. done.
-      }
-      apply elem_of_dom_2 with (x := da).
-      rewrite lookup_op.
-      assert (Hnone_new : mk_frag r 1 (ks ∖ {[k]}) !! x = None).
-      { rewrite /mk_frag lookup_singleton_ne; done. }
-      rewrite Hnone_new Hbf_lookup left_id //.
-  }
-
-  repeat split.
-  - rewrite map_Forall_lookup.
-    intros k0 v0 Hlookup0.
-    simpl in Hlookup0.
-    apply lookup_delete_Some in Hlookup0 as [_ Hlookup_old].
-    exact (map_Forall_lookup_1 _ _ _ _ Hobj Hlookup_old).
-  - intros r0 [dq agree_ks] Hb.
-    rewrite lookup_op in Hb.
-    destruct (decide (r0 = r)) as [->|Hneq].
-    + rewrite /mk_frag lookup_singleton_eq Hbf_none right_id in Hb.
-      inversion Hb; subst dq agree_ks. done.
-    + assert (Hlookup_new : mk_frag r 1 (ks ∖ {[k]}) !! r0 = None).
-      { rewrite /mk_frag lookup_singleton_ne; done. }
-      rewrite Hlookup_new in Hb.
-      rewrite left_id in Hb.
-      assert (Hlookup_old : (mk_frag r 1 ks ⋅ bf) !! r0 = Some (dq, agree_ks)).
-      { rewrite lookup_op.
-        assert (Hnone_old : mk_frag r 1 ks !! r0 = None).
-        { rewrite /mk_frag lookup_singleton_ne; done. }
-        rewrite Hnone_old Hb left_id //. }
-      exact (map_Forall_lookup_1
-        (λ _ '(dq0, _), ✓ dq0)
-        (mk_frag r 1 ks ⋅ bf) r0 (dq, agree_ks)
-        Hvalid Hlookup_old).
-  - intros r0 [dq agree_ks] Hb.
-    rewrite lookup_op in Hb.
-    destruct (decide (r0 = r)) as [->|Hneq].
-    + rewrite /mk_frag lookup_singleton_eq Hbf_none right_id in Hb.
-      inversion Hb; subst dq agree_ks.
-      exists (ks ∖ {[k]}). split; [done|].
-      assert (Hfdel :
-        filter (λ '(_, v0), f v0 = Some r) (delete k (proj_state a)) =
-        delete k (filter (λ '(_, v0), f v0 = Some r) (proj_state a))).
-      { apply map_filter_delete. }
-      rewrite Hfdel dom_delete_L Hks_dom. done.
-    + assert (Hlookup_new : mk_frag r 1 (ks ∖ {[k]}) !! r0 = None).
-      { rewrite /mk_frag lookup_singleton_ne; done. }
-      rewrite Hlookup_new in Hb.
-      rewrite left_id in Hb.
-      assert (Hlookup_old : (mk_frag r 1 ks ⋅ bf) !! r0 = Some (dq, agree_ks)).
-      { rewrite lookup_op.
-        assert (Hnone_old : mk_frag r 1 ks !! r0 = None).
-        { rewrite /mk_frag lookup_singleton_ne; done. }
-        rewrite Hnone_old Hb left_id //. }
-      destruct (Hchildren _ _ Hlookup_old) as (ks0 & Hagree & Hdom).
-      exists ks0. split; [done|].
-      assert (Hfdel :
-        filter (λ '(_, v0), f v0 = Some r0) (delete k (proj_state a)) =
-        filter (λ '(_, v0), f v0 = Some r0) (proj_state a)).
-      { change
-          ((filter (λ '(_, v0), f v0 = Some r0) (delete k (proj_state a)) : gmap K (leibnizO V)) =
-           (filter (λ '(_, v0), f v0 = Some r0) (proj_state a) : gmap K (leibnizO V))).
-        refine (@map_filter_delete_not K (gmap K)
-          _ _ _ _ _ _ _ _ _ (leibnizO V)
-          (λ '(_, v0), f v0 = Some r0) _ (proj_state a) k _).
-        intros y Hy.
-        rewrite Hak in Hy. inversion Hy; subst.
-        rewrite Hfkr. intros Hcontra.
-        inversion Hcontra. subst. done.
-      }
-      rewrite Hfdel. done.
-  - intros r0 da Hb.
-    destruct (decide (r0 = r)) as [->|Hneq].
-    + done.
-    + rewrite lookup_op in Hb.
-      assert (Hlookup_new : mk_frag r 1 (ks ∖ {[k]}) !! r0 = None).
-      { rewrite /mk_frag lookup_singleton_ne; done. }
-      rewrite Hlookup_new in Hb.
-      rewrite left_id in Hb.
-      assert (Hlookup_old : (mk_frag r 1 ks ⋅ bf) !! r0 = Some da).
-      { rewrite lookup_op.
-        assert (Hnone_old : mk_frag r 1 ks !! r0 = None).
-        { rewrite /mk_frag lookup_singleton_ne; done. }
-        rewrite Hnone_old Hb left_id //. }
-      eapply Hreferences; done.
-Qed.
-
-Lemma simple_update a k v v':
-  (proj_state a) !! k = Some v →
-  f v = f v' →
-  g k v = g k v' →
-  ●C a ~~> ●C ((<[k := v']> (proj_state a)), (proj_used_reference a)).
-Proof.
-  intros Hak Hfv Hg.
-  apply view_update_auth.
-  intros n bf [Hobj [Hvalid [Hchildren Hreferences]]].
-  repeat split.
-  - rewrite map_Forall_lookup.
-    intros k0 v0 Hlookup0.
-    simpl in Hlookup0.
-    destruct (decide (k0 = k)) as [->|Hneq_k].
-    + apply lookup_insert_Some in Hlookup0.
-      destruct Hlookup0 as [[_ Hv0]|[Hneq _]].
-      * symmetry in Hv0. subst v0.
-        rewrite <- Hg.
-        exact (map_Forall_lookup_1 _ _ _ _ Hobj Hak).
-      * exfalso. apply Hneq. reflexivity.
-    + apply lookup_insert_Some in Hlookup0.
-      destruct Hlookup0 as [[Heq _]|[_ Hlookup_old]].
-      * exfalso. apply Hneq_k. symmetry. exact Heq.
-      * exact (map_Forall_lookup_1 _ _ _ _ Hobj Hlookup_old).
-  - done.
-  - intros r [dq agree_ks] Hb.
-    destruct (Hchildren _ _ Hb) as (ks & Hagree & Hks).
-    exists ks. split; [exact Hagree|].
-    set (P := λ kv : K * V, f kv.2 = Some r).
-    assert (Hdom :
-      dom (filter P (<[k := v']> (proj_state a))) =
-      dom (filter P (proj_state a))).
-    { destruct (decide (P (k, v'))) as [HPv'|HPv'].
-      - assert (Hins :
-          filter P (<[k := v']> (proj_state a)) =
-          <[k := v']> (filter P (proj_state a))).
-        { apply (map_filter_insert_True P (proj_state a) k v'). done. }
-        rewrite Hins.
-        assert (HPv : P (k, v)).
-        { unfold P in *. rewrite Hfv. done. }
-        apply dom_insert_lookup_L.
-        eexists. apply map_lookup_filter_Some. split; [done|done].
-      - assert (Hins :
-          filter P (<[k := v']> (proj_state a)) =
-          filter P (proj_state a)).
-        { apply (map_filter_insert_not' P (proj_state a) k v').
-          - done.
-          - intros y Hy.
-            rewrite Hak in Hy. inversion Hy; subst.
-            unfold P in *. rewrite Hfv. done.
-        }
-        rewrite Hins. done.
+  apply map_eq. intros k.
+  unfold counted_reverse_index, counted_reversed_reference.reverse_index,
+    counted_reversed_reference.reference_count, extract_reference_count,
+    reverse_index.
+  rewrite map_lookup_imap lookup_gset_to_gmap.
+  destruct (state !! k) as [v|] eqn:Hlookup; simpl.
+  - rewrite lookup_gset_to_gmap.
+    assert (Hdom : k ∈ dom (filter (λ '(_, v0), r ∈ extract_reference_set v0) state) ↔
+      r ∈ extract_reference_set v).
+    { rewrite elem_of_dom. split.
+      - intros [v0 Hfilter].
+        apply map_lookup_filter_Some in Hfilter as [Hlookup0 Hr].
+        rewrite Hlookup in Hlookup0. inversion Hlookup0. done.
+      - intros Hr.
+        exists v. apply map_lookup_filter_Some. done.
     }
-    rewrite /P in Hdom.
-    rewrite Hdom. done.
-  - intros r da Hb.
-    eapply Hreferences; done.
-Qed.
-
-Lemma simple_create a k v cks:
-  (proj_state a) !! k = None →
-  f v = None →
-  dom (filter (λ '(_, v'), f v' = Some (g k v)) (proj_state a)) = cks →
-  g k v ∉ (proj_used_reference a) →
-  ●C a ~~>
-    ●C ((<[k := v]> (proj_state a)), ((proj_used_reference a) ∪ {[g k v]})) ⋅
-    ◯C (mk_frag (g k v) 1 cks).
-Proof.
-  intros Hak Hnone Hcks Hfresh.
-  apply view_update_alloc.
-  intros n bf [Hobj [Hvalid [Hchildren Hreferences]]].
-  assert (Hbf_none : bf !! (g k v) = None).
-  { destruct (bf !! (g k v)) as [da|] eqn:Hbf; [|done].
-    exfalso. apply Hfresh. eapply Hreferences; done.
-  }
-  assert (Hfilter :
-    ∀ r,
-      filter (λ '(_, v'), f v' = Some r) (<[k := v]> (proj_state a)) =
-      filter (λ '(_, v'), f v' = Some r) (proj_state a)).
-  { intros r.
-    change
-      ((filter (λ '(_, v'), f v' = Some r) (<[k := v]> (proj_state a)) : gmap K (leibnizO V)) =
-       (filter (λ '(_, v'), f v' = Some r) (proj_state a) : gmap K (leibnizO V))).
-    refine (@map_filter_insert_not' K (gmap K)
-      _ _ _ _ _ _ _ _ _ (leibnizO V)
-      (λ '(_, v'), f v' = Some r) _ (proj_state a) k v _ _).
-    - rewrite Hnone. discriminate.
-    - intros y Hy. rewrite Hak in Hy. done.
-  }
-  assert (Hdom_transfer :
-    ∀ x, x ∈ dom bf → x ∈ dom (mk_frag (g k v) 1 cks ⋅ bf)).
-  { intros x Hx.
-    destruct (decide (x = g k v)) as [->|Hneq_x].
-    - apply elem_of_dom_2 with (x := (DfracOwn 1, to_agree cks)).
-      rewrite lookup_op /mk_frag lookup_singleton_eq Hbf_none right_id //.
-    - rewrite elem_of_dom in Hx.
-      destruct Hx as [da Hlookup_bf].
-      apply elem_of_dom_2 with (x := da).
-      rewrite lookup_op.
-      assert (Hnone_new : mk_frag (g k v) 1 cks !! x = None).
-      { rewrite /mk_frag lookup_singleton_ne; done. }
-      rewrite Hnone_new Hlookup_bf left_id //.
-  }
-  repeat split.
-  - rewrite map_Forall_lookup.
-    intros k0 v0 Hlookup0.
-    simpl in Hlookup0.
-    destruct (decide (k0 = k)) as [->|Hneq_k].
-    + apply lookup_insert_Some in Hlookup0.
-      destruct Hlookup0 as [[_ Hv0]|[Hneq _]].
-      * symmetry in Hv0. subst v0.
-        apply elem_of_union. right.
-        apply elem_of_singleton. reflexivity.
-      * exfalso. apply Hneq. reflexivity.
-    + apply lookup_insert_Some in Hlookup0.
-      destruct Hlookup0 as [[Heq _]|[_ Hlookup_old]].
-      * exfalso. apply Hneq_k. symmetry. exact Heq.
-      * pose proof (map_Forall_lookup_1 _ _ _ _ Hobj Hlookup_old) as Hobj_used.
-        apply elem_of_union. left. exact Hobj_used.
-  - intros r [dq agree_ks] Hb.
-    rewrite lookup_op in Hb.
-    destruct (decide (r = g k v)) as [->|Hneq].
-    + rewrite /mk_frag lookup_singleton_eq Hbf_none right_id in Hb.
-      inversion Hb; subst dq agree_ks. done.
-    + rewrite /mk_frag in Hb.
-      assert (Hlookup_new : mk_frag (g k v) 1 cks !! r = None).
-      { rewrite /mk_frag lookup_singleton_ne; done. }
-      rewrite Hlookup_new in Hb.
-      rewrite left_id in Hb.
-      specialize (Hvalid _ _ Hb). done.
-  - intros r [dq agree_ks] Hb.
-    rewrite lookup_op in Hb.
-    destruct (decide (r = g k v)) as [->|Hneq].
-    + rewrite /mk_frag lookup_singleton_eq Hbf_none right_id in Hb.
-      inversion Hb; subst dq agree_ks.
-      exists cks. split; [done|].
-      rewrite (Hfilter (g k v)). done.
-    + rewrite /mk_frag in Hb.
-      assert (Hlookup_new : mk_frag (g k v) 1 cks !! r = None).
-      { rewrite /mk_frag lookup_singleton_ne; done. }
-      rewrite Hlookup_new in Hb.
-      rewrite left_id in Hb.
-      destruct (Hchildren _ _ Hb) as (ks & Hagree & Hdom).
-      exists ks. split; [done|].
-      rewrite (Hfilter r). done.
-  - intros r da Hb.
-    destruct (decide (r = g k v)) as [->|Hneq].
-    + set_solver.
-    + rewrite lookup_op in Hb.
-      assert (Hlookup_new : mk_frag (g k v) 1 cks !! r = None).
-      { rewrite /mk_frag lookup_singleton_ne; done. }
-      rewrite Hlookup_new in Hb.
-      rewrite left_id in Hb.
-      specialize (Hreferences _ _ Hb). set_solver.
-Qed.
-
-Lemma simple_delete a k v:
-  (proj_state a) !! k = Some v →
-  f v = None →
-  ●C a ~~> ●C ((delete k (proj_state a)), (proj_used_reference a)).
-Proof.
-  intros Hak Hnone.
-  apply view_update_auth.
-  intros n bf [Hobj [Hvalid [Hchildren Hreferences]]].
-  repeat split.
-  - rewrite map_Forall_lookup.
-    intros k0 v0 Hlookup0.
-    simpl in Hlookup0.
-    apply lookup_delete_Some in Hlookup0 as [_ Hlookup_old].
-    exact (map_Forall_lookup_1 _ _ _ _ Hobj Hlookup_old).
-  - done.
-  - intros r [dq agree_ks] Hb.
-    destruct (Hchildren _ _ Hb) as (ks & Hagree & Hks).
-    exists ks. split; [exact Hagree|].
-    assert (Hfilter :
-      filter (λ '(_, v'), f v' = Some r) (delete k (proj_state a)) =
-      filter (λ '(_, v'), f v' = Some r) (proj_state a)).
-    { change
-        ((filter (λ '(_, v'), f v' = Some r) (delete k (proj_state a)) : gmap K (leibnizO V)) =
-         (filter (λ '(_, v'), f v' = Some r) (proj_state a) : gmap K (leibnizO V))).
-      refine (@map_filter_delete_not K (gmap K)
-        _ _ _ _ _ _ _ _ _ (leibnizO V)
-        (λ '(_, v'), f v' = Some r) _ (proj_state a) k _).
-      intros y Hy.
-      rewrite Hak in Hy. inversion Hy; subst.
-      rewrite Hnone. discriminate.
-    }
-    rewrite Hfilter. done.
-  - intros r da Hb.
-    eapply Hreferences; done.
+    destruct (decide (r ∈ extract_reference_set v)) as [Hr|Hnot];
+      destruct (decide (k ∈ dom (filter (λ '(_, v0), r ∈ extract_reference_set v0) state))) as [Hk|Hknot];
+      simpl.
+    + rewrite (option_guard_True (r ∈ extract_reference_set v) (Some 1) Hr).
+      rewrite (option_guard_True
+        (k ∈ dom (filter (λ '(_, v0), r ∈ extract_reference_set v0) state))
+        (Some 1) Hk).
+      simpl. destruct (decide (0 < 1)%nat); [reflexivity|lia].
+    + exfalso. apply Hknot. by apply Hdom.
+    + exfalso. apply Hnot. by apply Hdom.
+    + rewrite (option_guard_False (r ∈ extract_reference_set v) Hnot).
+      rewrite (option_guard_False
+        (k ∈ dom (filter (λ '(_, v0), r ∈ extract_reference_set v0) state))
+        Hknot).
+      done.
+  - destruct (decide (k ∈ dom (filter (λ '(_, v0), r ∈ extract_reference_set v0) state))) as [Hk|Hk].
+    + exfalso.
+      apply elem_of_dom in Hk as [v Hfilter].
+      apply map_lookup_filter_Some in Hfilter as [Hlookup0 _].
+      rewrite Hlookup in Hlookup0. done.
+    + rewrite (option_guard_False
+        (k ∈ dom (filter (λ '(_, v0), r ∈ extract_reference_set v0) state))
+        Hk).
+      done.
 Qed.
 
 Class reversed_referenceG Σ :=
-  { #[global] reversed_reference_inG :: inG Σ (viewR view_rel); }.
+  { #[global] reversed_reference_countedG ::
+      @counted_reversed_reference.counted_reversed_referenceG
+        K _ _ R _ _ V extract_reference_count to_reference Σ; }.
 
 Definition reversed_referenceΣ :=
-  #[GFunctor (viewR view_rel)].
+  @counted_reversed_reference.counted_reversed_referenceΣ
+    K _ _ R _ _ V extract_reference_count to_reference.
 
 #[global]
 Instance subG_reversed_referenceG Σ :
   subG reversed_referenceΣ Σ → reversed_referenceG Σ.
-Proof. solve_inG. Qed.
+Proof.
+  intros Hsub.
+  constructor.
+  exact (@counted_reversed_reference.subG_counted_reversed_referenceG
+    K _ _ R _ _ V extract_reference_count to_reference Σ Hsub).
+Qed.
 
 Context `{!reversed_referenceG Σ}.
 
-Global Instance own_auth_timeless γ a : Timeless (own γ (●C a)).
-Proof. apply _. Qed.
-
-Global Instance own_frag_timeless γ b : Timeless (own γ (◯C b)).
-Proof. apply _. Qed.
-
 Definition own_auth γ (state: gmap K V) (used_reference: gset R) : iProp Σ :=
-  own γ (●C (state, used_reference)).
+  @counted_reversed_reference.own_auth
+    K _ _ R _ _ V extract_reference_count to_reference Σ _
+    γ (state, used_reference).
 
 Definition own_frag γ r dq ks : iProp Σ :=
-  own γ (◯C (mk_frag r dq ks)).
+  @counted_reversed_reference.own_frag
+    K _ _ R _ _ V extract_reference_count to_reference Σ _
+    γ r dq (gset_to_gmap 1 ks).
+
+Global Instance own_auth_timeless γ state used_reference :
+  Timeless (own_auth γ state used_reference).
+Proof. apply _. Qed.
+
+Global Instance own_frag_timeless γ r dq ks :
+  Timeless (own_frag γ r dq ks).
+Proof. apply _. Qed.
+
+Definition map_reverse_index (state : gmap K V) (r : R) : gset K :=
+  dom (filter (λ '(_, v), r ∈ extract_reference_set v) state).
+
+Local Lemma map_raw_reverse_index_eq state r :
+  @counted_reversed_reference.reverse_index
+    K _ _ R _ _ V extract_reference_count state r =
+    gset_to_gmap 1 (map_reverse_index state r).
+Proof.
+  apply counted_reverse_index_eq.
+Qed.
 
 Lemma own_auth_frag_valid {γ state used_reference r dq ks}:
   own_auth γ state used_reference -∗
   own_frag γ r dq ks -∗
-  ⌜ ks = dom (filter (λ '(_, v), f v = Some r) state) ⌝ ∗
+  ⌜ ks = map_reverse_index state r ⌝ ∗
   ⌜ r ∈ used_reference ⌝.
 Proof.
+  unfold own_auth, own_frag.
   iIntros "Hauth Hfrag".
-  iDestruct (own_valid_2 with "Hauth Hfrag") as "Hvalid".
-  iDestruct (internal_cmra_valid_elim with "Hvalid") as %Hvalid0.
-  iPureIntro.
-  rewrite /own_auth /own_frag in Hvalid0.
-  pose proof (proj1 (view_both_validN view_rel 0%nat
-    (state, used_reference) (mk_frag r dq ks)) Hvalid0) as Hrel0.
-  assert (Hvalid : ✓ (●C (state, used_reference) ⋅ ◯C (mk_frag r dq ks))).
-  { rewrite /cview_auth /cview_frag.
-    apply (proj2 (view_both_valid view_rel (state, used_reference) (mk_frag r dq ks))).
-    intros n. exact Hrel0.
-  }
-  pose proof (auth_frag_valid (state, used_reference) r dq ks Hvalid) as [Hks Hr].
-  split; done.
+  iDestruct (@counted_reversed_reference.own_auth_frag_valid
+    K _ _ R _ _ V extract_reference_count to_reference Σ _
+    γ (state, used_reference) r dq (gset_to_gmap 1 ks)
+    with "Hauth Hfrag") as "[%Hks %Hr]".
+  iPureIntro. split; [|done].
+  simpl in Hks.
+  rewrite map_raw_reverse_index_eq in Hks.
+  apply (f_equal dom) in Hks.
+  rewrite !dom_gset_to_gmap in Hks.
+  done.
+Qed.
+
+Local Lemma dom_filter_insert_preserve
+    (m : gmap K V) k v v' r :
+  m !! k = Some v →
+  (r ∈ extract_reference_set v' ↔ r ∈ extract_reference_set v) →
+  map_reverse_index (<[k := v']> m) r = map_reverse_index m r.
+Proof.
+  intros Hlookup Hiff.
+  apply set_eq. intros k0.
+  rewrite /map_reverse_index !elem_of_dom.
+  split.
+  - intros [v0 Hlookup0].
+    apply map_lookup_filter_Some in Hlookup0 as [Hlookup0 Hr0].
+    destruct (decide (k0 = k)) as [->|Hneq].
+    + rewrite lookup_insert_eq in Hlookup0. inversion Hlookup0; subst v0.
+      exists v. apply map_lookup_filter_Some. split; [done|].
+      exact (proj1 Hiff Hr0).
+    + apply lookup_insert_Some in Hlookup0 as [[Heq _]|[_ Hlookup0]].
+      * done.
+      * exists v0. apply map_lookup_filter_Some. done.
+  - intros [v0 Hlookup0].
+    apply map_lookup_filter_Some in Hlookup0 as [Hlookup0 Hr0].
+    destruct (decide (k0 = k)) as [->|Hneq].
+    + rewrite Hlookup in Hlookup0. inversion Hlookup0; subst v0.
+      exists v'. apply map_lookup_filter_Some. split.
+      * rewrite lookup_insert_eq. done.
+      * exact (proj2 Hiff Hr0).
+    + exists v0. apply map_lookup_filter_Some. split; [|done].
+      rewrite lookup_insert_ne; done.
+Qed.
+
+Local Lemma map_reverse_index_insert_new_singleton state k v r :
+  state !! k = None →
+  r ∈ extract_reference_set v →
+  map_reverse_index (<[k := v]> state) r =
+    map_reverse_index state r ∪ {[k]}.
+Proof.
+  intros Hlookup Hr.
+  rewrite /map_reverse_index.
+  replace (filter (λ '(_, v0), r ∈ extract_reference_set v0) (<[k:=v]> state))
+    with (<[k:=v]> (filter (λ '(_, v0), r ∈ extract_reference_set v0) state)).
+  2:{ symmetry. apply map_filter_insert_True. exact Hr. }
+  rewrite dom_insert_L. Timeout 10 set_solver.
+Qed.
+
+Local Lemma map_reverse_index_insert_new_not state k v r :
+  state !! k = None →
+  r ∉ extract_reference_set v →
+  map_reverse_index (<[k := v]> state) r = map_reverse_index state r.
+Proof.
+  intros Hlookup Hr.
+  rewrite /map_reverse_index.
+  apply f_equal.
+  apply map_filter_insert_not'; [done|].
+  intros y Hy. rewrite Hlookup in Hy. done.
+Qed.
+
+Local Lemma map_reverse_index_insert_add state k v v' r :
+  state !! k = Some v →
+  r ∉ extract_reference_set v →
+  r ∈ extract_reference_set v' →
+  map_reverse_index (<[k := v']> state) r =
+    map_reverse_index state r ∪ {[k]}.
+Proof.
+  intros Hlookup Hnotin Hin.
+  apply set_eq. intros k0.
+  rewrite /map_reverse_index elem_of_union !elem_of_dom elem_of_singleton.
+  split.
+  - intros [v0 Hlookup0].
+    apply map_lookup_filter_Some in Hlookup0 as [Hlookup0 Hr0].
+    destruct (decide (k0 = k)) as [->|Hneq].
+    + right. done.
+    + left. exists v0. apply map_lookup_filter_Some. split; [|done].
+      rewrite lookup_insert_ne in Hlookup0; done.
+  - intros Hk0.
+    destruct Hk0 as [[v0 Hlookup0]|Heq]; [|subst k0].
+    + apply map_lookup_filter_Some in Hlookup0 as [Hlookup0 Hr0].
+      exists v0. apply map_lookup_filter_Some. split; [|done].
+      destruct (decide (k0 = k)) as [->|Hneq].
+      * rewrite Hlookup in Hlookup0. inversion Hlookup0. subst v0.
+        exfalso. apply Hnotin. done.
+      * rewrite lookup_insert_ne; done.
+    + exists v'. apply map_lookup_filter_Some. split; [|done].
+      rewrite lookup_insert_eq. done.
+Qed.
+
+Local Lemma map_reverse_index_insert_remove state k v v' r :
+  state !! k = Some v →
+  r ∈ extract_reference_set v →
+  extract_reference_set v' = extract_reference_set v ∖ {[r]} →
+  map_reverse_index (<[k := v']> state) r =
+    map_reverse_index state r ∖ {[k]}.
+Proof.
+  intros Hlookup Hr Hrefs.
+  apply set_eq. intros k0.
+  rewrite /map_reverse_index elem_of_difference !elem_of_dom elem_of_singleton.
+  split.
+  - intros [v0 Hlookup0].
+    apply map_lookup_filter_Some in Hlookup0 as [Hlookup0 Hr0].
+    destruct (decide (k0 = k)) as [->|Hneq].
+    + rewrite lookup_insert_eq in Hlookup0. inversion Hlookup0. subst v0.
+      rewrite Hrefs in Hr0. apply elem_of_difference in Hr0 as [_ Hnot].
+      exfalso. apply Hnot. apply elem_of_singleton. done.
+    + apply lookup_insert_Some in Hlookup0 as [[Heq _]|[_ Hlookup0]]; [done|].
+      split; [|done].
+      exists v0. apply map_lookup_filter_Some. done.
+  - intros [[v0 Hlookup0] Hneq].
+    apply map_lookup_filter_Some in Hlookup0 as [Hlookup0 Hr0].
+    exists v0. apply map_lookup_filter_Some. split; [|done].
+    rewrite lookup_insert_ne; done.
+Qed.
+
+Local Lemma map_reverse_index_delete_singleton state k v r :
+  state !! k = Some v →
+  extract_reference_set v = {[r]} →
+  map_reverse_index (delete k state) r =
+    map_reverse_index state r ∖ {[k]}.
+Proof.
+  intros Hlookup Hrefs.
+  apply set_eq. intros k0.
+  rewrite /map_reverse_index elem_of_difference !elem_of_dom elem_of_singleton.
+  split.
+  - intros [v0 Hlookup0].
+    apply map_lookup_filter_Some in Hlookup0 as [Hlookup0 Hr0].
+    apply lookup_delete_Some in Hlookup0 as [Hneq Hlookup0].
+    split; [|done].
+    exists v0. apply map_lookup_filter_Some. done.
+  - intros [[v0 Hlookup0] Hneq].
+    apply map_lookup_filter_Some in Hlookup0 as [Hlookup0 Hr0].
+    exists v0. apply map_lookup_filter_Some. split; [|done].
+    apply lookup_delete_Some. done.
+Qed.
+
+Local Lemma map_reverse_index_delete_not state k r :
+  k ∉ map_reverse_index state r →
+  map_reverse_index (delete k state) r = map_reverse_index state r.
+Proof.
+  intros Hnotin.
+  apply set_eq. intros k0.
+  rewrite /map_reverse_index !elem_of_dom.
+  split.
+  - intros [v0 Hlookup0].
+    apply map_lookup_filter_Some in Hlookup0 as [Hlookup0 Hr0].
+    apply lookup_delete_Some in Hlookup0 as [_ Hlookup0].
+    exists v0. apply map_lookup_filter_Some. done.
+  - intros [v0 Hlookup0].
+    apply map_lookup_filter_Some in Hlookup0 as [Hlookup0 Hr0].
+    destruct (decide (k0 = k)) as [->|Hneq].
+    + exfalso. apply Hnotin.
+      rewrite /map_reverse_index elem_of_dom.
+      exists v0. apply map_lookup_filter_Some. done.
+    + exists v0. apply map_lookup_filter_Some. split; [|done].
+      apply lookup_delete_Some. done.
+Qed.
+
+Local Lemma map_reverse_index_delete_singleton_other state k v r r0 :
+  state !! k = Some v →
+  extract_reference_set v = {[r]} →
+  r0 ≠ r →
+  map_reverse_index (delete k state) r0 = map_reverse_index state r0.
+Proof.
+  intros Hlookup Hrefs Hneq.
+  apply map_reverse_index_delete_not.
+  intros Hk.
+  rewrite /map_reverse_index elem_of_dom in Hk.
+  destruct Hk as [v0 Hfilter].
+  apply map_lookup_filter_Some in Hfilter as [Hlookup0 Hr0].
+  rewrite Hlookup in Hlookup0. inversion Hlookup0. subst v0.
+  rewrite Hrefs in Hr0. apply elem_of_singleton in Hr0. done.
 Qed.
 
 Lemma create_reference_vs {γ state used_reference r ks} k v cks:
   state !! k = None →
-  f v = Some r →
-  g k v ≠ r → (* No self-parenting *)
-  dom (filter (λ '(_, v'), f v' = Some (g k v)) state) = cks →
-  g k v ∉ used_reference →
+  extract_reference_set v = {[r]} →
+  to_reference k v ≠ r →
+  map_reverse_index state (to_reference k v) = cks →
+  to_reference k v ∉ used_reference →
   own_auth γ state used_reference -∗
   own_frag γ r 1 ks ==∗
-    own_auth γ (<[k := v]> state) (used_reference ∪ {[g k v]}) ∗
+    own_auth γ (<[k := v]> state) (used_reference ∪ {[to_reference k v]}) ∗
     own_frag γ r 1 (ks ∪ {[k]}) ∗
-    own_frag γ (g k v) 1 cks.
+    own_frag γ (to_reference k v) 1 cks.
 Proof.
-  iIntros (Hak Hfr Hnself Hcks Hfresh) "Hauth Hfrag".
+  iIntros (Hak Hrefs Hnself Hcks Hfresh) "Hauth Hfrag".
+  iPoseProof (own_auth_frag_valid with "Hauth Hfrag") as "[%Hks %Hr_used]".
+  unfold own_auth, own_frag.
   iMod (own_update_2 with "Hauth Hfrag") as "H".
-  { eapply create_reference; done. }
+  { eapply (@counted_reversed_reference.generic_reference_update_alloc_reference_from_old_obj
+      K _ _ R _ _ V extract_reference_count to_reference)
+      with (a := (state, used_reference))
+           (a' := (<[k := v]> state, used_reference ∪ {[to_reference k v]}))
+           (r := r)
+           (ks := gset_to_gmap 1 ks)
+           (ks' := gset_to_gmap 1 (ks ∪ {[k]}))
+           (new_r := to_reference k v)
+           (new_ks := gset_to_gmap 1 cks).
+    - exact Hfresh.
+    - intros Heq. apply Hnself. symmetry. exact Heq.
+    - intros Hobj.
+      rewrite map_Forall_lookup.
+      intros k0 v0 Hlookup0.
+      simpl in Hlookup0.
+      destruct (decide (k0 = k)) as [->|Hneq].
+      + apply lookup_insert_Some in Hlookup0 as [[_ Hv0]|[Hneq' _]].
+        * symmetry in Hv0. subst v0. Timeout 10 set_solver.
+        * exfalso. apply Hneq'. done.
+      + apply lookup_insert_Some in Hlookup0 as [[Heq _]|[_ Hlookup_old]].
+        * exfalso. apply Hneq. symmetry. done.
+        * pose proof (map_Forall_lookup_1 _ _ _ _ Hobj Hlookup_old) as Hused.
+          Timeout 10 set_solver.
+    - Timeout 10 set_solver.
+    - Timeout 10 set_solver.
+    - rewrite map_raw_reverse_index_eq.
+      assert (Hri :
+        map_reverse_index (<[k:=v]> state) r =
+        map_reverse_index state r ∪ {[k]}).
+      { apply map_reverse_index_insert_new_singleton; [done|].
+        rewrite Hrefs. apply elem_of_singleton. done. }
+      rewrite Hri. subst ks. done.
+    - rewrite map_raw_reverse_index_eq.
+      assert (Hri :
+        map_reverse_index (<[k:=v]> state) (to_reference k v) =
+        map_reverse_index state (to_reference k v)).
+      { apply map_reverse_index_insert_new_not; [done|].
+        rewrite Hrefs. intros Hin. apply elem_of_singleton in Hin. done. }
+      rewrite Hri Hcks. done.
+    - intros r0 Hneq Hr0. Timeout 10 set_solver.
+    - intros r0 Hneq Hr0.
+      rewrite !map_raw_reverse_index_eq.
+      assert (Hri :
+        map_reverse_index (<[k:=v]> state) r0 =
+        map_reverse_index state r0).
+      { apply map_reverse_index_insert_new_not; [done|].
+        rewrite Hrefs. intros Hin. apply elem_of_singleton in Hin. done. }
+      rewrite Hri. done.
+  }
   iModIntro.
-  iDestruct (own_op with "H") as "[H Hfrag2]".
-  iDestruct (own_op with "H") as "[Hauth Hfrag1]".
+  iDestruct (own_op with "H") as "[H Hfrag_new]".
+  iDestruct (own_op with "H") as "[Hauth Hfrag]".
   iFrame.
 Qed.
 
 Lemma set_reference_vs {γ state used_reference r ks} k v v':
   state !! k = Some v →
-  f v = None →
-  f v' = Some r →
-  g k v = g k v' →
+  r ∉ extract_reference_set v →
+  extract_reference_set v' = extract_reference_set v ∪ {[r]} →
+  to_reference k v = to_reference k v' →
   own_auth γ state used_reference -∗ own_frag γ r 1 ks ==∗
     own_auth γ (<[k := v']> state) used_reference ∗ own_frag γ r 1 (ks ∪ {[k]}).
 Proof.
-  iIntros (Hak Hnone Hfr Hg) "Hauth Hfrag".
+  iIntros (Hak Hnotin Hrefs Hg) "Hauth Hfrag".
+  iPoseProof (own_auth_frag_valid with "Hauth Hfrag") as "[%Hks %Hr_used]".
+  unfold own_auth, own_frag.
   iMod (own_update_2 with "Hauth Hfrag") as "H".
-  { eapply set_reference; done. }
-  iModIntro.
-  iDestruct (own_op with "H") as "[Hauth Hfrag]".
-  iFrame.
+  { eapply (@counted_reversed_reference.generic_reference_update_from_old_obj
+      K _ _ R _ _ V extract_reference_count to_reference)
+      with (a := (state, used_reference))
+           (a' := (<[k := v']> state, used_reference))
+           (r := r)
+           (ks := gset_to_gmap 1 ks)
+           (ks' := gset_to_gmap 1 (ks ∪ {[k]})).
+    - intros Hobj.
+      rewrite map_Forall_lookup.
+      intros k0 v0 Hlookup0.
+      simpl in Hlookup0.
+      destruct (decide (k0 = k)) as [->|Hneq].
+      + apply lookup_insert_Some in Hlookup0 as [[_ Hv0]|[Hneq' _]].
+        * symmetry in Hv0. subst v0. rewrite <- Hg.
+          exact (map_Forall_lookup_1 _ _ _ _ Hobj Hak).
+        * exfalso. apply Hneq'. done.
+      + apply lookup_insert_Some in Hlookup0 as [[Heq _]|[_ Hlookup_old]].
+        * exfalso. apply Hneq. symmetry. done.
+        * exact (map_Forall_lookup_1 _ _ _ _ Hobj Hlookup_old).
+    - exact Hr_used.
+    - rewrite map_raw_reverse_index_eq.
+      assert (Hri :
+        map_reverse_index (<[k:=v']> state) r =
+        map_reverse_index state r ∪ {[k]}).
+      { apply (map_reverse_index_insert_add state k v v' r); [done|done|].
+        rewrite Hrefs. Timeout 10 set_solver. }
+      rewrite Hri. subst ks. done.
+    - done.
+    - intros r0 Hneq Hr0.
+      rewrite !map_raw_reverse_index_eq.
+      assert (Hri :
+        map_reverse_index (<[k:=v']> state) r0 =
+        map_reverse_index state r0).
+      { apply (dom_filter_insert_preserve state k v v' r0); [done|].
+        rewrite Hrefs. split; intros Hin.
+        - apply elem_of_union in Hin as [Hin|Hin]; [done|].
+          apply elem_of_singleton in Hin. subst. done.
+        - apply elem_of_union. left. done. }
+      rewrite Hri. done.
+  }
+  iModIntro. iDestruct (own_op with "H") as "[Hauth Hfrag]". iFrame.
 Qed.
 
 Lemma unset_reference_vs {γ state used_reference r ks} k v v':
   state !! k = Some v →
-  f v = Some r →
-  f v' = None →
-  g k v = g k v' →
+  r ∈ extract_reference_set v →
+  extract_reference_set v' = extract_reference_set v ∖ {[r]} →
+  to_reference k v = to_reference k v' →
   own_auth γ state used_reference -∗ own_frag γ r 1 ks ==∗
     own_auth γ (<[k := v']> state) used_reference ∗ own_frag γ r 1 (ks ∖ {[k]}).
 Proof.
-  iIntros (Hak Hfr Hnone Hg) "Hauth Hfrag".
+  iIntros (Hak Hin Hrefs Hg) "Hauth Hfrag".
+  iPoseProof (own_auth_frag_valid with "Hauth Hfrag") as "[%Hks %Hr_used]".
+  unfold own_auth, own_frag.
   iMod (own_update_2 with "Hauth Hfrag") as "H".
-  { eapply unset_reference; done. }
-  iModIntro.
-  iDestruct (own_op with "H") as "[Hauth Hfrag]".
-  iFrame.
+  { eapply (@counted_reversed_reference.generic_reference_update_from_old_obj
+      K _ _ R _ _ V extract_reference_count to_reference)
+      with (a := (state, used_reference))
+           (a' := (<[k := v']> state, used_reference))
+           (r := r)
+           (ks := gset_to_gmap 1 ks)
+           (ks' := gset_to_gmap 1 (ks ∖ {[k]})).
+    - intros Hobj.
+      rewrite map_Forall_lookup.
+      intros k0 v0 Hlookup0.
+      simpl in Hlookup0.
+      destruct (decide (k0 = k)) as [->|Hneq].
+      + apply lookup_insert_Some in Hlookup0 as [[_ Hv0]|[Hneq' _]].
+        * symmetry in Hv0. subst v0. rewrite <- Hg.
+          exact (map_Forall_lookup_1 _ _ _ _ Hobj Hak).
+        * exfalso. apply Hneq'. done.
+      + apply lookup_insert_Some in Hlookup0 as [[Heq _]|[_ Hlookup_old]].
+        * exfalso. apply Hneq. symmetry. done.
+        * exact (map_Forall_lookup_1 _ _ _ _ Hobj Hlookup_old).
+    - exact Hr_used.
+    - rewrite map_raw_reverse_index_eq.
+      assert (Hri :
+        map_reverse_index (<[k:=v']> state) r =
+        map_reverse_index state r ∖ {[k]}).
+      { apply (map_reverse_index_insert_remove state k v v' r); done. }
+      rewrite Hri. subst ks. done.
+    - done.
+    - intros r0 Hneq Hr0.
+      rewrite !map_raw_reverse_index_eq.
+      assert (Hri :
+        map_reverse_index (<[k:=v']> state) r0 =
+        map_reverse_index state r0).
+      { apply (dom_filter_insert_preserve state k v v' r0); [done|].
+        rewrite Hrefs. split; intros Hin0.
+        - apply elem_of_difference in Hin0 as [Hin0 _]. done.
+        - apply elem_of_difference. split; [done|].
+          intros Heq. apply elem_of_singleton in Heq. subst. done. }
+      rewrite Hri. done.
+  }
+  iModIntro. iDestruct (own_op with "H") as "[Hauth Hfrag]". iFrame.
 Qed.
 
 Lemma delete_reference_vs {γ state used_reference r ks} k v:
   state !! k = Some v →
-  f v = Some r →
+  extract_reference_set v = {[r]} →
   own_auth γ state used_reference -∗ own_frag γ r 1 ks ==∗
     own_auth γ (delete k state) used_reference ∗ own_frag γ r 1 (ks ∖ {[k]}).
 Proof.
-  iIntros (Hak Hfr) "Hauth Hfrag".
+  iIntros (Hak Hrefs) "Hauth Hfrag".
+  iPoseProof (own_auth_frag_valid with "Hauth Hfrag") as "[%Hks %Hr_used]".
+  unfold own_auth, own_frag.
   iMod (own_update_2 with "Hauth Hfrag") as "H".
-  { eapply delete_reference; done. }
-  iModIntro.
-  iDestruct (own_op with "H") as "[Hauth Hfrag]".
-  iFrame.
+  { eapply (@counted_reversed_reference.generic_reference_update_from_old_obj
+      K _ _ R _ _ V extract_reference_count to_reference)
+      with (a := (state, used_reference))
+           (a' := (delete k state, used_reference))
+           (r := r)
+           (ks := gset_to_gmap 1 ks)
+           (ks' := gset_to_gmap 1 (ks ∖ {[k]})).
+    - intros Hobj.
+      rewrite map_Forall_lookup.
+      intros k0 v0 Hlookup0.
+      simpl in Hlookup0.
+      apply lookup_delete_Some in Hlookup0 as [_ Hlookup0].
+      exact (map_Forall_lookup_1 _ _ _ _ Hobj Hlookup0).
+    - exact Hr_used.
+    - rewrite map_raw_reverse_index_eq.
+      assert (Hri :
+        map_reverse_index (delete k state) r =
+        map_reverse_index state r ∖ {[k]}).
+      { apply (map_reverse_index_delete_singleton state k v r); done. }
+      rewrite Hri. subst ks. done.
+    - done.
+    - intros r0 Hneq Hr0.
+      rewrite !map_raw_reverse_index_eq.
+      assert (Hri :
+        map_reverse_index (delete k state) r0 =
+        map_reverse_index state r0).
+      { apply (map_reverse_index_delete_singleton_other state k v r r0); done. }
+      rewrite Hri. done.
+  }
+  iModIntro. iDestruct (own_op with "H") as "[Hauth Hfrag]". iFrame.
 Qed.
 
 Lemma delete_reference_vs2 {γ state used_reference r ks} k:
   k ∈ ks →
+  (∀ v, r ∈ extract_reference_set v → extract_reference_set v = {[r]}) →
   own_auth γ state used_reference -∗ own_frag γ r 1 ks ==∗
     own_auth γ (delete k state) used_reference ∗ own_frag γ r 1 (ks ∖ {[k]}).
 Proof.
-  iIntros (Hk) "Hauth Hfrag".
-  iMod (own_update_2 with "Hauth Hfrag") as "H".
-  { eapply delete_reference2; done. }
-  iModIntro.
-  iDestruct (own_op with "H") as "[Hauth Hfrag]".
-  iFrame.
+  iIntros (Hk Hsingleton) "Hauth Hfrag".
+  iPoseProof (own_auth_frag_valid with "Hauth Hfrag") as "[%Hks %Hr_used]".
+  assert (∃ v, state !! k = Some v ∧ r ∈ extract_reference_set v) as (v & Hak & Hr).
+  { rewrite Hks /map_reverse_index elem_of_dom in Hk.
+    destruct Hk as [v Hfilter].
+    apply map_lookup_filter_Some in Hfilter as [Hak Hr].
+    eauto.
+  }
+  iApply (delete_reference_vs k v with "Hauth Hfrag"); [done|].
+  apply Hsingleton. done.
 Qed.
 
 Lemma simple_update_vs {γ state used_reference} k v v':
   state !! k = Some v →
-  f v = f v' →
-  g k v = g k v' →
+  extract_reference_set v = extract_reference_set v' →
+  to_reference k v = to_reference k v' →
   own_auth γ state used_reference ==∗ own_auth γ (<[k := v']> state) used_reference.
 Proof.
-  iIntros (Hak Hf Hg) "Hauth".
+  iIntros (Hak Hrefs Hg) "Hauth".
+  unfold own_auth.
   iMod (own_update with "Hauth") as "Hauth".
-  { eapply simple_update; done. }
+  { eapply (@counted_reversed_reference.generic_update_from_old_obj
+      K _ _ R _ _ V extract_reference_count to_reference)
+      with (a := (state, used_reference))
+           (a' := (<[k := v']> state, used_reference)).
+    - intros Hobj.
+      rewrite map_Forall_lookup.
+      intros k0 v0 Hlookup0.
+      simpl in Hlookup0.
+      destruct (decide (k0 = k)) as [->|Hneq].
+      + apply lookup_insert_Some in Hlookup0 as [[_ Hv0]|[Hneq' _]].
+        * symmetry in Hv0. subst v0. rewrite <- Hg.
+          exact (map_Forall_lookup_1 _ _ _ _ Hobj Hak).
+        * exfalso. apply Hneq'. done.
+      + apply lookup_insert_Some in Hlookup0 as [[Heq _]|[_ Hlookup_old]].
+        * exfalso. apply Hneq. symmetry. done.
+        * exact (map_Forall_lookup_1 _ _ _ _ Hobj Hlookup_old).
+    - done.
+    - intros r0 Hr0.
+      rewrite !map_raw_reverse_index_eq.
+      assert (Hri :
+        map_reverse_index (<[k:=v']> state) r0 =
+        map_reverse_index state r0).
+      { apply (dom_filter_insert_preserve state k v v' r0); [done|].
+        rewrite Hrefs. done. }
+      rewrite Hri. done.
+  }
   iModIntro. iExact "Hauth".
 Qed.
 
 Lemma simple_create_vs {γ state used_reference} k v cks:
   state !! k = None →
-  f v = None →
-  dom (filter (λ '(_, v'), f v' = Some (g k v)) state) = cks →
-  g k v ∉ used_reference →
+  extract_reference_set v = ∅ →
+  map_reverse_index state (to_reference k v) = cks →
+  to_reference k v ∉ used_reference →
   own_auth γ state used_reference ==∗
-    own_auth γ (<[k := v]> state) (used_reference ∪ {[g k v]}) ∗
-    own_frag γ (g k v) 1 cks.
+    own_auth γ (<[k := v]> state) (used_reference ∪ {[to_reference k v]}) ∗
+    own_frag γ (to_reference k v) 1 cks.
 Proof.
-  iIntros (Hak Hnone Hcks Hfresh) "Hauth".
+  iIntros (Hak Hrefs Hcks Hfresh) "Hauth".
+  unfold own_auth, own_frag.
   iMod (own_update with "Hauth") as "H".
-  { eapply simple_create; done. }
+  { eapply (@counted_reversed_reference.generic_alloc_reference_from_old_obj
+      K _ _ R _ _ V extract_reference_count to_reference)
+      with (a := (state, used_reference))
+           (a' := (<[k := v]> state, used_reference ∪ {[to_reference k v]}))
+           (r := to_reference k v)
+           (ks := gset_to_gmap 1 cks).
+    - exact Hfresh.
+    - intros Hobj.
+      rewrite map_Forall_lookup.
+      intros k0 v0 Hlookup0.
+      simpl in Hlookup0.
+      destruct (decide (k0 = k)) as [->|Hneq].
+      + apply lookup_insert_Some in Hlookup0 as [[_ Hv0]|[Hneq' _]].
+        * symmetry in Hv0. subst v0. Timeout 10 set_solver.
+        * exfalso. apply Hneq'. done.
+      + apply lookup_insert_Some in Hlookup0 as [[Heq _]|[_ Hlookup_old]].
+        * exfalso. apply Hneq. symmetry. done.
+        * pose proof (map_Forall_lookup_1 _ _ _ _ Hobj Hlookup_old) as Hused.
+          Timeout 10 set_solver.
+    - Timeout 10 set_solver.
+    - rewrite map_raw_reverse_index_eq.
+      assert (Hri :
+        map_reverse_index (<[k:=v]> state) (to_reference k v) =
+        map_reverse_index state (to_reference k v)).
+      { apply map_reverse_index_insert_new_not; [done|].
+        rewrite Hrefs. Timeout 10 set_solver. }
+      rewrite Hri Hcks. done.
+    - intros r0 Hr0. Timeout 10 set_solver.
+    - intros r0 Hr0.
+      rewrite !map_raw_reverse_index_eq.
+      assert (Hri :
+        map_reverse_index (<[k:=v]> state) r0 =
+        map_reverse_index state r0).
+      { apply map_reverse_index_insert_new_not; [done|].
+        rewrite Hrefs. Timeout 10 set_solver. }
+      rewrite Hri. done.
+  }
   iModIntro.
   iDestruct (own_op with "H") as "[Hauth Hfrag]".
   iFrame.
@@ -1313,12 +656,37 @@ Qed.
 
 Lemma simple_delete_vs {γ state used_reference} k v:
   state !! k = Some v →
-  f v = None →
+  extract_reference_set v = ∅ →
   own_auth γ state used_reference ==∗ own_auth γ (delete k state) used_reference.
 Proof.
-  iIntros (Hak Hnone) "Hauth".
+  iIntros (Hak Hrefs) "Hauth".
+  unfold own_auth.
   iMod (own_update with "Hauth") as "Hauth".
-  { eapply simple_delete; done. }
+  { eapply (@counted_reversed_reference.generic_update_from_old_obj
+      K _ _ R _ _ V extract_reference_count to_reference)
+      with (a := (state, used_reference))
+           (a' := (delete k state, used_reference)).
+    - intros Hobj.
+      rewrite map_Forall_lookup.
+      intros k0 v0 Hlookup0.
+      simpl in Hlookup0.
+      apply lookup_delete_Some in Hlookup0 as [_ Hlookup0].
+      exact (map_Forall_lookup_1 _ _ _ _ Hobj Hlookup0).
+    - done.
+    - intros r0 Hr0.
+      rewrite !map_raw_reverse_index_eq.
+      assert (Hri :
+        map_reverse_index (delete k state) r0 =
+        map_reverse_index state r0).
+      { apply map_reverse_index_delete_not.
+        intros Hk.
+        rewrite /map_reverse_index elem_of_dom in Hk.
+        destruct Hk as [v0 Hfilter].
+        apply map_lookup_filter_Some in Hfilter as [Hlookup Hr].
+        rewrite Hak in Hlookup. inversion Hlookup. subst v0.
+        rewrite Hrefs in Hr. Timeout 10 set_solver. }
+      rewrite Hri. done.
+  }
   iModIntro. iExact "Hauth".
 Qed.
 
