src/proof/iam_model/algebra/ghost_map_wrapper.v
@@ -1,0 +1,82 @@
+From New.proof Require Import prelude.
+From New.ghost Require Import ghost_map.
+From New.proof.iam_model Require Export aliases.
+
+Section ghost_map_wrapper.
+Context {ext : ffi_syntax} {go_gctx : GoGlobalContext}.
+Context `{!allG Σ}.
+
+Definition own_identity_auth γ (identities : identity_map) : iProp Σ :=
+  ghost_map_auth (K:=iammodel.IdentityID.t) (V:=gmap iammodel.PolicyID.t unit) γ 1 identities.
+
+Definition own_identity_frag
+    γ (identity : iammodel.IdentityID.t) (policy_ids : gmap iammodel.PolicyID.t unit) : iProp Σ :=
+  ghost_map_elem (K:=iammodel.IdentityID.t) (V:=gmap iammodel.PolicyID.t unit)
+    γ identity DfracDiscarded policy_ids.
+
+Definition own_policy_auth γ (policies : policy_map) : iProp Σ :=
+  ghost_map_auth (K:=iammodel.PolicyID.t) (V:=iammodel.IdentityPolicy.t) γ 1 policies.
+
+Definition own_policy_frag
+    γ (policy_id : iammodel.PolicyID.t) (policy : iammodel.IdentityPolicy.t) : iProp Σ :=
+  ghost_map_elem (K:=iammodel.PolicyID.t) (V:=iammodel.IdentityPolicy.t)
+    γ policy_id DfracDiscarded policy.
+
+Global Instance own_identity_auth_timeless γ identities :
+  Timeless (own_identity_auth γ identities).
+Proof. unfold own_identity_auth. apply _. Qed.
+
+Global Instance own_identity_frag_timeless γ identity policy_ids :
+  Timeless (own_identity_frag γ identity policy_ids).
+Proof. unfold own_identity_frag. apply _. Qed.
+
+Global Instance own_identity_frag_persistent γ identity policy_ids :
+  Persistent (own_identity_frag γ identity policy_ids).
+Proof. unfold own_identity_frag. apply _. Qed.
+
+Global Instance own_policy_auth_timeless γ policies :
+  Timeless (own_policy_auth γ policies).
+Proof. unfold own_policy_auth. apply _. Qed.
+
+Global Instance own_policy_frag_timeless γ policy_id policy :
+  Timeless (own_policy_frag γ policy_id policy).
+Proof. unfold own_policy_frag. apply _. Qed.
+
+Global Instance own_policy_frag_persistent γ policy_id policy :
+  Persistent (own_policy_frag γ policy_id policy).
+Proof. unfold own_policy_frag. apply _. Qed.
+
+Lemma own_identity_auth_frag_lookup {γ identities identity policy_ids} :
+  own_identity_auth γ identities -∗
+  own_identity_frag γ identity policy_ids -∗
+  ⌜ identities !! identity = Some policy_ids ⌝.
+Proof.
+  unfold own_identity_auth, own_identity_frag.
+  iIntros "Hauth Hfrag".
+  iDestruct (ghost_map_lookup with "Hauth Hfrag") as %Hlookup.
+  done.
+Qed.
+
+Lemma own_policy_auth_frag_lookup {γ policies policy_id policy} :
+  own_policy_auth γ policies -∗
+  own_policy_frag γ policy_id policy -∗
+  ⌜ policies !! policy_id = Some policy ⌝.
+Proof.
+  unfold own_policy_auth, own_policy_frag.
+  iIntros "Hauth Hfrag".
+  iDestruct (ghost_map_lookup with "Hauth Hfrag") as %Hlookup.
+  done.
+Qed.
+
+Lemma own_policy_insert_vs {γ policies policy_id policy} :
+  policies !! policy_id = None →
+  own_policy_auth γ policies ==∗
+    own_policy_auth γ (<[policy_id := policy]> policies) ∗
+    own_policy_frag γ policy_id policy.
+Proof.
+  unfold own_policy_auth, own_policy_frag.
+  iIntros (Hfresh) "Hauth".
+  iMod (ghost_map_insert_persist policy_id policy with "Hauth") as "[$ $]"; done.
+Qed.
+
+End ghost_map_wrapper.
