src/proof/iam_model/aliases.v
@@ -1,0 +1,12 @@
+From New.proof Require Import prelude.
+From New.code Require Export iam_model.
+From iris.algebra Require Import gmap.
+
+Definition identity_map : Type :=
+  gmap iammodel.IdentityID.t (gmap iammodel.PolicyID.t unit).
+
+Definition policy_map {ext : ffi_syntax} {go_gctx : GoGlobalContext} : Type :=
+  gmap iammodel.PolicyID.t iammodel.IdentityPolicy.t.
+
+Definition policy_id_set : Type :=
+  gmap iammodel.PolicyID.t unit.
