iam_model/go.mod
@@ -1,0 +1,3 @@
+module iam_model
+
+go 1.24.2
